git-svn-id: https://webdav.seas.upenn.edu/svn/sol/vol@3654 eef5ea85-cc2e-0410-bd84-0fae1f012da8

src/Transforms/dae.v
@@ -19,6 +19,7 @@ Require Import palloca_props.
 Require Import memory_props.
 Require Import sb_msim.
 Require Import sb_ds_gv_inject.
+Require Import sb_metadata.
 
 Definition fdef_simulation (pinfo: PhiInfo) f1 f2 : Prop :=
   if (fdef_dec (PI_f pinfo) f1) then 
@@ -127,17 +128,19 @@ match ECs1, ECs2 with
 | _, _ => False
 end.
 
-Definition isnt_alloca_in_ECs (pinfo:PhiInfo) (ecs:list Opsem.ExecutionContext) 
+Definition isnt_alloca_in_ECs (pinfo:PhiInfo) (ecs:list (fdef*Opsem.GVsMap)) 
   (blk:mblock) : Prop :=
-  forall ec0 (Hin: In ec0 ecs), 
-    is_alloca_in_EC pinfo (Opsem.CurFunction ec0) (Opsem.Locals ec0) blk = false.
+  forall f lc (Hin: In (f,lc) ecs), 
+    is_alloca_in_EC pinfo f lc blk = false.
 
-Definition Mem_simulation (pinfo:PhiInfo) mgb (mi:MoreMem.meminj)
-  (ecs:list Opsem.ExecutionContext) Mem1 Mem2 : Prop :=
+Definition strip_ECs (ecs:list (@Opsem.ExecutionContext DGVs))
+  : list (fdef*Opsem.GVsMap) :=
+List.map (fun ec => (Opsem.CurFunction ec, Opsem.Locals ec)) ecs.
+
+Definition mem_simulation (pinfo:PhiInfo) mgb (mi:MoreMem.meminj)
+  (ecs:list (fdef*Opsem.GVsMap)) Mem1 Mem2 : Prop :=
 MoreMem.mem_inj mi Mem1 Mem2 /\
-(forall blk, 
-   (isnt_alloca_in_ECs pinfo ecs blk -> mi blk <> None) /\
-   ~ isnt_alloca_in_ECs pinfo ecs blk -> mi blk = None) /\
+(forall blk, ~ isnt_alloca_in_ECs pinfo ecs blk -> mi blk = None) /\
 wf_sb_mi mgb mi Mem1 Mem2.
 
 (* Copied from sb_ds_sim *)
@@ -157,7 +160,7 @@ match (St1, St2) with
     products_simulation pinfo Ps1 Ps2 /\
     ECs_simulation pinfo mi ECs1 ECs2 /\
     gl1 = gl2 /\ ftable_simulation mi fs1 fs2 /\ 
-    Mem_simulation pinfo mgb mi ECs1 M1 M2
+    mem_simulation pinfo mgb mi (strip_ECs ECs1) M1 M2
 end.
 
 Definition removable_State (pinfo: PhiInfo) (St:@Opsem.State DGVs) : Prop :=
@@ -206,7 +209,12 @@ repeat match goal with
 | H1 : ?f ?a ?b = _,
   H2 : ?f ?a ?b = _ |- _ =>
   rewrite H1 in H2; inv H2
+| H1 : ?f ?a = _,
+  H2 : ?f ?a = _ |- _ =>
+  rewrite H1 in H2; inv H2
 | H1 : _ @ _ |- _ => inv H1
+| H : ?f _ = ?f _ |- _ => inv H
+| H : False |- _ => inv H
 end.
 
 Lemma cmds_simulation_nil_inv: forall pinfo f1 cs,
@@ -260,7 +268,6 @@ match goal with
   destruct c'; tinv HBinF1'; clear HBinF1'
 end.
 
-
 Lemma fdef_sim__block_sim : forall pinfo f1 f2 b1 b2 l0,
   fdef_simulation pinfo f1 f2 ->
   lookupBlockViaLabelFromFdef f1 l0 = Some b1 ->
@@ -284,129 +291,12 @@ Proof.
   destruct (fdef_dec (PI_f pinfo) F); inv H; auto.
 Qed.
 
-(*
-Lemma no_alias_head_tail_update : 
-  forall pinfo ptr EC1 EC2 ECs
-  (EQ: Opsem.CurFunction EC1 = Opsem.CurFunction EC2)
-  (Hp: forall gvsa
-   (Hlkup: lookupAL (GVsT DGVs) (Opsem.Locals EC2) (PI_id pinfo) = ret gvsa),
-   lookupAL (GVsT DGVs) (Opsem.Locals EC1) (PI_id pinfo) = ret gvsa)
-  (Hnalias: no_alias_head_tail pinfo ptr (EC1 :: ECs)),
-  no_alias_head_tail pinfo ptr (EC2 :: ECs).
-Proof.
-  intros.
-  unfold no_alias_head_tail in *.
-  intros.
-  simpl in Hin.
-  destruct Hin as [Hin | Hin]; subst.
-    assert (no_alias_head_in_tail pinfo ptr EC1) as J. 
-      apply Hnalias; simpl; auto.
-    clear Hnalias.
-    unfold no_alias_head_in_tail in *. simpl in *. intros. 
-    rewrite Heq in EQ.
-    apply J; auto.
-
-    apply Hnalias; simpl; auto.
-Qed.
-
-Lemma switchToNewBasicBlock_sim : forall TD l1 l2 ps cs1 cs2 tmn1 tmn2 B1 B2 
-  gl lc lc1 lc2 F pinfo
-  (H23 : @Opsem.switchToNewBasicBlock DGVs TD
-          (block_intro l1 ps cs1 tmn1) B1 gl lc = 
-         ret lc1)
-  (Hbsim2 : block_simulation pinfo F B1 B2)
-  (H2 : Opsem.switchToNewBasicBlock TD
-         (block_intro l2 ps cs2 tmn2) B2 gl lc = 
-        ret lc2), lc1 = lc2.
-Admitted.
-
-Lemma mem_simulation_update_locals : 
-  forall pinfo TD EC1 EC2 ECs M1 M2
-  (EQ: Opsem.CurFunction EC1 = Opsem.CurFunction EC2)
-  (Hp: forall gvsa
-   (Hlkup: lookupAL (GVsT DGVs) (Opsem.Locals EC1) (PI_id pinfo) = ret gvsa),
-   lookupAL (GVsT DGVs) (Opsem.Locals EC2) (PI_id pinfo) = ret gvsa)
-  (Hmsim: Mem_simulation pinfo TD (EC1 :: ECs) M1 M2),
-  Mem_simulation pinfo TD (EC2 :: ECs) M1 M2.
-Proof.
-  intros.
-  destruct Hmsim as [Hmsim1 Hmsim2].
-  split; auto.
-    intros.
-    eapply Hmsim2 with (ptr:=ptr)(ty:=ty)(al:=al); eauto.
-    eapply no_alias_head_tail_update in Hnalias; eauto; simpl; auto.
-Qed.
-
-Lemma mstore_palloca_Mem_simulation: forall TD M1 mp2 gv1 a M1' pinfo lc2 gl2
-  B1 cs1 tmn2 als2 ECs1 M2 i0 t v
-  (H23: mstore TD M1 mp2 t gv1 a = ret M1')
-  (H20: @Opsem.getOperandValue DGVs TD (value_id (PI_id pinfo)) lc2 gl2 =
-          ret mp2)
-  (Hmsim: Mem_simulation pinfo TD
-            ({|
-             Opsem.CurFunction := PI_f pinfo;
-             Opsem.CurBB := B1;
-             Opsem.CurCmds := insn_store i0 t v (value_id (PI_id pinfo)) a
-                              :: cs1;
-             Opsem.Terminator := tmn2;
-             Opsem.Locals := lc2;
-             Opsem.Allocas := als2 |} :: ECs1) M1 M2),
-  Mem_simulation pinfo TD
-            ({|
-             Opsem.CurFunction := PI_f pinfo;
-             Opsem.CurBB := B1;
-             Opsem.CurCmds := cs1;
-             Opsem.Terminator := tmn2;
-             Opsem.Locals := lc2;
-             Opsem.Allocas := als2 |} :: ECs1) M1' M2.
-Proof.
-  intros.
-  destruct Hmsim as [Hmsim1 Hmsim2].
-  split.
-    apply MemProps.nextblock_mstore in H23.
-    rewrite <- H23. auto.
-
-    intros. 
-    eapply Hmsim2; eauto using no_alias_head_tail_irrel.
-    eapply MemProps.mstore_preserves_mload_inv'; eauto.
-    assert (no_alias_head_in_tail pinfo ptr 
-              {| Opsem.CurFunction := PI_f pinfo;
-                 Opsem.CurBB := B1;
-                 Opsem.CurCmds := cs1;
-                 Opsem.Terminator := tmn2;
-                 Opsem.Locals := lc2;
-                 Opsem.Allocas := als2 |}) as J.
-      apply Hnalias; simpl; auto.
-    apply MemProps.no_alias_sym.
-    unfold no_alias_head_in_tail in J; eauto.
-Qed.
-
-Ltac repeat_solve :=
-  repeat (match goal with
-          | |- Mem_simulation _ _ _ _ _ => idtac 
-          | |- _ => split; eauto 2 using cmds_at_block_tail_next
-          end).
-*)
-
 Lemma products_simulation__fdef_simulation : forall pinfo Ps1 Ps2 fid f1 f2,
   lookupFdefViaIDFromProducts Ps2 fid = Some f2 ->
   lookupFdefViaIDFromProducts Ps1 fid = Some f1 ->
   products_simulation pinfo Ps1 Ps2 ->
   fdef_simulation pinfo f1 f2.
 Admitted.
-
-Lemma lookupFdefViaPtr__simulation : forall pinfo Ps1 Ps2 fptr f1 f2 fs,
-  OpsemAux.lookupFdefViaPtr Ps2 fs fptr = Some f2 ->
-  products_simulation pinfo Ps1 Ps2 ->
-  OpsemAux.lookupFdefViaPtr Ps1 fs fptr = Some f1 ->
-  fdef_simulation pinfo f1 f2.
-Proof.
-  intros.
-  unfold OpsemAux.lookupFdefViaPtr in *.
-  remember (OpsemAux.lookupFdefViaGVFromFunTable fs fptr) as R2.
-  destruct R2 as [fid|]; inv H1. simpl in H.
-  eapply products_simulation__fdef_simulation in H0; eauto.
-Qed.
 
 Lemma fdef_simulation__entry_block_simulation: forall pinfo F1 F2 B1 B2,
   fdef_simulation pinfo F1 F2 ->
@@ -422,96 +312,919 @@ Lemma fdef_simulation_inv: forall pinfo fh1 fh2 bs1 bs2,
     (fun b1 b2 => block_simulation pinfo (fdef_intro fh1 bs1) b1 b2) bs1 bs2.
 Admitted.
 
-Lemma lookupFdefViaPtr__simulation_l2r : forall pinfo Ps1 Ps2 fptr f1 fs,
-  products_simulation pinfo Ps1 Ps2 ->
-  OpsemAux.lookupFdefViaPtr Ps1 fs fptr = Some f1 ->
-  exists f2, 
-    OpsemAux.lookupFdefViaPtr Ps2 fs fptr = Some f2 /\
-    fdef_simulation pinfo f1 f2.
-Admitted.
-
-Lemma lookupExFdecViaPtr__simulation_l2r : forall pinfo Ps1 Ps2 fptr f fs,
-  products_simulation pinfo Ps1 Ps2 ->
-  OpsemAux.lookupExFdecViaPtr Ps1 fs fptr = Some f ->
-  OpsemAux.lookupExFdecViaPtr Ps2 fs fptr = Some f.
-Admitted.
-(*
-Lemma no_alias_head_tail_cons_and: forall pinfo ptr EC ECs,
-  no_alias_head_tail pinfo ptr (EC :: ECs) ->
-  no_alias_head_in_tail pinfo ptr EC /\ no_alias_head_tail pinfo ptr ECs.
-Proof.
-  intros.
-  unfold no_alias_head_tail in *.  
-  split.
-    apply H; simpl; auto.
-    intros. apply H; simpl; auto.
-Qed.
-*)
-
-Lemma callExternalFunction__Mem_simulation: forall pinfo mi St1 M1 M2 fid0 gvss0
-  oresult1 M1' oresult2 M2' mgb,
-  Mem_simulation pinfo mgb mi St1 M1 M2 ->
-  OpsemAux.callExternalFunction M1 fid0 gvss0 = ret (oresult1, M1') ->
-  OpsemAux.callExternalFunction M2 fid0 gvss0 = ret (oresult2, M2') ->
-  oresult1 = oresult2 /\ 
-  exists mi', 
-    Mem_simulation pinfo mgb mi' St1 M1' M2' /\ Values.inject_incr mi mi'.
-Admitted.
-(*
-Ltac dse_is_sim_common_case :=
-match goal with
-| Hcssim2: cmds_simulation _ _ _ _,
-  Hop2: Opsem.sInsn _ _ _ _,
-  Hmsim: Mem_simulation _ _ _ _ _ |- _ =>
-  apply cmds_simulation_nelim_cons_inv in Hcssim2; simpl; auto;
-  destruct Hcssim2 as [cs3' [Heq Hcssim2]]; subst;
-  inv Hop2; uniq_result;
-  repeat_solve;
-    eapply mem_simulation_update_locals in Hmsim; simpl; try solve [
-      eauto |
-      simpl; intros;
-      match goal with
-      | Hlkup : lookupAL _ ?lc ?id1 = Some ?gvsa |-
-        lookupAL _ (updateAddAL _ ?lc _ _ ) ?id1 = Some ?gvsa => 
-        admit  (* id <> palloca *)
-      end]
-end.
-*)  
-
-Lemma mem_simulation__palloca : forall mi TD Mem1 Mem2 tsz gn Mem1' mb B1
-  v cs1 tmn1 als1 ECs1 pinfo maxb lc1
-  (Hmsim : Mem_simulation pinfo maxb mi
-            ({|
-             Opsem.CurFunction := PI_f pinfo;
-             Opsem.CurBB := B1;
-             Opsem.CurCmds := insn_alloca (PI_id pinfo) 
-                                (PI_typ pinfo) v (PI_align pinfo) :: cs1;
-             Opsem.Terminator := tmn1;
-             Opsem.Locals := lc1;
-             Opsem.Allocas := als1 |} :: ECs1) Mem1 Mem2)
-  (Hmlc: malloc TD Mem1 tsz gn (PI_align pinfo) = ret (Mem1', mb)),
-  exists mi',
-    Mem_simulation pinfo maxb mi'
-            ({|
-             Opsem.CurFunction := PI_f pinfo;
-             Opsem.CurBB := B1;
-             Opsem.CurCmds := cs1;
-             Opsem.Terminator := tmn1;
-             Opsem.Locals := 
-               updateAddAL (GVsT DGVs) lc1 (PI_id pinfo)
-                 ($ blk2GV TD mb # typ_pointer (PI_typ pinfo) $);
-             Opsem.Allocas := mb :: als1 |} :: ECs1) Mem1' Mem2 /\
-    Values.inject_incr mi mi' /\
-    mi' mb = None /\
-    (forall b, b <> mb -> mi b = mi' b).
-Admitted.
-
 Ltac repeat_solve :=
   repeat (match goal with
-          | |- Mem_simulation _ _ _ _ _ _ => idtac 
+          | |- mem_simulation _ _ _ _ _ _ => idtac 
           | |- _ => split; eauto 2 using cmds_at_block_tail_next
           end).
 
+Ltac zeauto := eauto with zarith.
+
+Lemma mem_simulation__palloca : forall mi TD Mem1 Mem2 tsz gn Mem1' mb 
+  ECs1 pinfo maxb lc1
+  (Hmsim : mem_simulation pinfo maxb mi
+            ((PI_f pinfo, lc1) :: ECs1) Mem1 Mem2)
+  (Hmlc: malloc TD Mem1 tsz gn (PI_align pinfo) = ret (Mem1', mb)),
+  exists mi',
+    mem_simulation pinfo maxb mi'
+            ((PI_f pinfo, 
+               updateAddAL (GVsT DGVs) lc1 (PI_id pinfo)
+                 ($ blk2GV TD mb # typ_pointer (PI_typ pinfo) $))
+             :: ECs1) Mem1' Mem2 /\
+    Values.inject_incr mi mi' /\
+    mi' mb = None /\
+    (forall b, b <> mb -> mi b = mi' b).
+Proof.
+  intros.
+  unfold malloc in *.
+  inv_mbind'. symmetry_ctx.
+  destruct (zle 0 (Size.to_Z tsz * z)); tinv H0.
+  remember (Mem.alloc Mem1 0 (Size.to_Z tsz * z)) as R.
+  inv H0.
+  assert (Hresult := H1). apply Mem.alloc_result in Hresult. subst.
+  assert (Hnext := H1). apply Mem.nextblock_alloc in Hnext.
+  assert (Hvalid := H1). apply Mem.valid_new_block in Hvalid.
+  destruct Hmsim as [Hmsim1 [Hmsim2 Hmsim3]].
+  exists (fun b => if zeq b (Mem.nextblock Mem1) then None else mi b).
+  assert (inject_incr mi 
+           (fun b : Z => if zeq b (Mem.nextblock Mem1) then None else mi b))
+    as Hinject_incr.
+    unfold inject_incr.
+    intros b b' d H.
+    destruct (zeq b (Mem.nextblock Mem1)); subst; auto.
+      destruct Hmsim3 as [_ _ Hmap1 _].
+      assert (mi (Mem.nextblock Mem1) = None) as J.
+        apply Hmap1; auto with zarith.
+      uniq_result.
+
+  repeat_solve.
+Case "mem_sim".
+    split.
+  SCase "mem_inj".
+    clear Hmsim2 Hmsim3.
+    destruct Hmsim1.
+    apply MoreMem.mk_mem_inj.
+    SSCase "mi_access".
+      intros b1 b2 d c ofs p J1 J2.
+      destruct (zeq b1 (Mem.nextblock Mem1)); subst; tinv J1.
+      eapply Mem.valid_access_alloc_inv with (b:=(Mem.nextblock Mem1))(lo:=0)
+        (hi:=Size.to_Z tsz * z)(p:=p) in J2; eauto.
+      destruct (eq_block); subst; try solve [eauto | contradict n; auto].
+
+    SSCase "mi_memval".
+Transparent Mem.alloc.
+      intros b1 ofs b2 d J1 J2.
+      injection H1. intro MEM.
+      destruct Mem1. destruct Mem1'. destruct Mem2. 
+      inv MEM. clear H1 Hnext Hvalid.
+      simpl in *.
+      unfold Mem.perm in *. simpl in *.
+      clear maxaddress_pos0 conversion_props0.
+      unfold update.     
+      destruct (zeq b1 nextblock); subst; tinv J1.
+      apply MoreMem.memval_inject_incr with (f:=mi); auto.
+      apply mi_memval; auto.
+        clear - J2 n.
+        unfold update in J2.
+        destruct (zeq b1 nextblock); subst; 
+          try solve [auto | contradict n; auto].
+Opaque Mem.alloc.
+
+    split.
+  SCase "isnt_alloca_in_ECs".
+    clear Hmsim1 Hmsim3 Hinject_incr.
+    intros.
+    destruct (zeq blk (Mem.nextblock Mem1)); subst; auto.
+    apply Hmsim2. clear Hmsim2.
+    intro J. apply H. clear H.
+    unfold isnt_alloca_in_ECs in *.
+    intros.
+    simpl in Hin.
+    destruct Hin as [Hin | Hin]; subst.
+      inv Hin. simpl. unfold is_alloca_in_EC.
+      destruct (fdef_dec (PI_f pinfo) ); try congruence.
+      rewrite lookupAL_updateAddAL_eq.
+      rewrite Promotability.simpl_blk2GV.
+      destruct (Z_eq_dec (Mem.nextblock Mem1) blk); try congruence.
+
+      apply J. simpl; auto.
+
+  SCase "wfmi".
+    clear Hmsim1 Hmsim2 Hinject_incr.
+    destruct Hmsim3 as [Hno_overlap Hnull Hmap1 Hmap2 mi_freeblocks 
+      mi_mappedblocks mi_range_block mi_bounds mi_globals].
+    split.
+    SSCase "no_overlap".
+      clear - Hno_overlap Hnext Hmap2.
+      unfold MoreMem.meminj_no_overlap in *.
+      intros.      
+      destruct (zeq b1 (Mem.nextblock Mem1)); subst.
+        destruct (zeq b2 (Mem.nextblock Mem1)); subst; try congruence.
+        destruct (zeq b2 (Mem.nextblock Mem1)); subst; eauto; try congruence.
+    SSCase "null".
+      destruct (zeq Mem.nullptr (Mem.nextblock Mem1)); subst; auto.
+        assert(J':=@Mem.nextblock_pos Mem1).
+        rewrite <- e in J'.
+        unfold Mem.nullptr in J'.
+        contradict J'; omega.
+    SSCase "map1".
+      intros b H2.
+      rewrite Hnext in H2.
+      destruct (zeq b (Mem.nextblock Mem1)); subst; zeauto.
+    SSCase "map2".
+      intros b1 b delta2 J'.
+      destruct (zeq b1 (Mem.nextblock Mem1)); tinv J'; eauto.
+    SSCase "freeblocks".
+      intros b J'.
+      destruct (zeq b (Mem.nextblock Mem1)); subst.
+        contradict H1; auto.
+
+        apply mi_freeblocks.
+          intro J1. apply J'.
+          eapply Mem.valid_block_alloc; eauto.
+    SSCase "mappedblocks".
+      intros b b' delta J'.
+      destruct (zeq b (Mem.nextblock Mem1)); subst; eauto; try congruence.
+    SSCase "range_block".
+      intros b b' delta J'.
+      destruct (zeq b (Mem.nextblock Mem1)); inv J'; subst; eauto.
+    SSCase "bounds".
+      intros b b' delta J'.
+      erewrite Mem.bounds_alloc; eauto.
+      unfold eq_block.
+      destruct (zeq b (Mem.nextblock Mem1)); subst; eauto; try congruence.
+    SSCase "globals".
+      intros b J'.
+      destruct (zeq b (Mem.nextblock Mem1)); subst; eauto.
+        assert (J'':=J').
+        apply mi_globals in J'.
+        destruct (SBspecMetadata.valid_block_dec Mem1 (Mem.nextblock Mem1)).
+          apply Mem.fresh_block_alloc in H1.
+          contradict H1; auto.
+     
+          apply mi_freeblocks in n.        
+          rewrite n in J'. inversion J'.
+
+Case "mi_prop1".
+    destruct (zeq (Mem.nextblock Mem1) (Mem.nextblock Mem1)); congruence.
+
+Case "mi_prop2".
+    intros.
+    destruct (zeq b (Mem.nextblock Mem1)); subst; congruence.
+Qed.
+
+Lemma reg_simulation_update_palloca: forall (pinfo : PhiInfo) 
+  (mi : MoreMem.meminj) TD (lc1 lc2 : Opsem.GVsMap)
+  (Hlcsim2 : reg_simulation pinfo mi (PI_f pinfo) lc1 lc2)
+  (mb : mblock) (mi' : MoreMem.meminj)
+  (Hinc : inject_incr mi mi'),
+  reg_simulation pinfo mi' (PI_f pinfo)
+    (updateAddAL (GVsT DGVs) lc1 (PI_id pinfo)
+       ($ blk2GV TD mb # typ_pointer (PI_typ pinfo) $)) lc2.
+Proof.
+  intros.
+  unfold reg_simulation in *.
+  destruct (fdef_dec (PI_f pinfo) (PI_f pinfo)); try congruence.
+  intros.
+  assert (J:=@Hlcsim2 i0). clear Hlcsim2.
+  destruct (id_dec (PI_id pinfo) i0); subst; auto.
+  intros.
+  rewrite <- lookupAL_updateAddAL_neq in H; auto.
+  eapply J in H; eauto.
+  eapply gv_inject_incr; eauto.
+Qed.
+
+Lemma inject_incr__preserves__als_simulation: forall pinfo mi f lc1 als1 als2 
+  mi',
+  als_simulation pinfo mi f lc1 als1 als2 ->
+  (forall blk, 
+    is_alloca_in_EC pinfo f lc1 blk = true -> 
+    mi blk = None -> mi' blk = None) ->
+  inject_incr mi mi' ->
+  als_simulation pinfo mi' f lc1 als1 als2.
+Proof.
+  induction als1; destruct als2; simpl; intros; auto.
+    remember (is_alloca_in_EC pinfo f lc1 a) as R.
+    destruct R; auto.
+    destruct H.
+    split; eauto.
+
+    remember (is_alloca_in_EC pinfo f lc1 a) as R.
+    destruct R; destruct H; split; eauto.
+Qed.
+
+Lemma inject_incr__preserves__reg_simulation: forall pinfo mi f lc1 lc2 mi',
+  reg_simulation pinfo mi f lc1 lc2 ->
+  inject_incr mi mi' ->
+  reg_simulation pinfo mi' f lc1 lc2. 
+Proof.
+  intros pinfo mi f lc1 lc2 mi' Hrsim Hinc.
+  unfold reg_simulation in *.
+  destruct (fdef_dec (PI_f pinfo) f); subst.
+    intros.
+    assert (J:=@Hrsim i0).
+    destruct (id_dec (PI_id pinfo) i0); subst; auto.
+    intros. eapply J in H; eauto using gv_inject_incr.
+
+    intros. eapply Hrsim in H; eauto using gv_inject_incr.
+Qed.
+
+Lemma inject_incr__preserves__EC_simulation: forall pinfo mi mi' EC1 EC2,
+  EC_simulation pinfo mi EC1 EC2 ->
+  (forall blk, 
+    is_alloca_in_EC pinfo (Opsem.CurFunction EC1) (Opsem.Locals EC1) blk 
+      = true -> 
+    mi blk = None -> mi' blk = None) ->
+  inject_incr mi mi' ->
+  EC_simulation pinfo mi' EC1 EC2.
+Proof.
+  intros.
+  destruct EC1 as [f1 b1 cs1 tmn1 lc1 als1].
+  destruct EC2 as [f2 b2 cs2 tmn2 lc2 als2].
+  destruct f1. destruct f2.
+  destruct b1; tinv H.
+  unfold EC_simulation in H.
+  destruct H as [Hfsim [Heq0 [Hasim [Hbsim [Heqb1 [Heqb2 [Hrsim Hcssim]]]]]]]; 
+    subst.
+  eapply inject_incr__preserves__als_simulation in Hasim; eauto.
+  eapply inject_incr__preserves__reg_simulation in Hrsim; eauto.
+  repeat (split; auto).
+Qed.
+
+Lemma inject_incr__preserves__ECs_simulation: forall pinfo mi mi' ECs1 ECs2,
+  ECs_simulation pinfo mi ECs1 ECs2 ->
+  (forall blk, ~ isnt_alloca_in_ECs pinfo (strip_ECs ECs1) blk ->
+    mi blk = None -> mi' blk = None) ->
+  inject_incr mi mi' ->
+  ECs_simulation pinfo mi' ECs1 ECs2.
+Proof.
+  induction ECs1; destruct ECs2; simpl; intros; auto.
+    destruct H as [J1 J2].
+    split.
+      eapply inject_incr__preserves__EC_simulation; eauto.
+        intros.
+        apply H0; auto.
+        intro J.
+        unfold isnt_alloca_in_ECs in J.
+        assert (In (Opsem.CurFunction a, Opsem.Locals a) 
+          ((Opsem.CurFunction a, Opsem.Locals a)::strip_ECs ECs1)) as G.
+          simpl. auto.
+        apply J in G. uniq_result.
+ 
+        apply IHECs1; auto.
+        intros. apply H0; auto.
+        intro J. apply H.
+        unfold isnt_alloca_in_ECs in *.
+        intros. apply J. simpl; auto.
+Qed.
+
+(* copied from sb_ds_trans_axiom.v *)
+Axiom inject_incr__preserves__ftable_simulation: forall mi mi' fs1 fs2,
+  ftable_simulation mi fs1 fs2 ->
+  inject_incr mi mi' ->
+  ftable_simulation mi' fs1 fs2.
+
+Ltac destruct_ctx_return :=
+match goal with
+| Hwfpp : OpsemPP.wf_State
+            {|
+            OpsemAux.CurSystem := _;
+            OpsemAux.CurTargetData := ?TD;
+            OpsemAux.CurProducts := _;
+            OpsemAux.Globals := _;
+            OpsemAux.FunTable := _
+             |} _,
+  Hnoalias : Promotability.wf_State _ _ _ _,
+  Hsim : State_simulation _ _ _ _ _ ?Cfg2 ?St2 ,
+  Hop2 : Opsem.sInsn _ _ _ _ |- _ =>
+  destruct TD as [los nts];
+  destruct Hwfpp as 
+    [Hwfg [HwfSystem [HmInS [_ [
+     [Hreach1 [HBinF1 [HFinPs1 _]]] 
+     [ 
+       [
+         [Hreach2 [HBinF2 [HFinPs2 _]]]
+         _
+       ]
+       HwfCall'
+     ]]
+    ]]]]; subst;
+  destruct Cfg2 as [S2 TD2 Ps2 gl2 fs2];
+  destruct St2 as [ECs2 M2];
+  simpl in Hsim;
+  destruct Hsim as [EQ1 [Hpsim [Hstksim [EQ2 [EQ3 Hmsim]]]]]; subst;
+  destruct ECs2 as [|[F2 B2 cs2 tmn2 lc2 als2] ECs2]; tinv Hstksim;
+  destruct Hstksim as [Hecsim Hstksim];
+  destruct ECs2 as [|[F3 B3 cs3 tmn3 lc3 als3] ECs2]; tinv Hstksim;
+  destruct Hstksim as [Hecsim' Hstksim];
+  unfold EC_simulation in Hecsim;
+  destruct Hecsim as 
+      [Hfsim2 [Heq1 [Halsim2 [Hbsim2 
+        [Heq3 [Heq4 [Hlcsim2 Hcssim2]]]]]]]; subst;
+  destruct Hecsim' as 
+      [Hfsim2' [Heq1' [Halsim2' [Hbsim2' 
+        [Heq3' [Heq4' [Hlcsim2' Hcssim2']]]]]]]; subst;
+  destruct Hnoalias as 
+    [
+      [[Hinscope1' _] [[[Hinscope2' _] [HwfECs' _]] _]] 
+      [[Hdisjals _] HwfM]
+    ]; simpl in Hdisjals;
+  fold Promotability.wf_ECStack in HwfECs';
+  apply cmds_simulation_nil_inv in Hcssim2; subst;
+  wfCall_inv
+end.
+
+(* The sb_ds_trans_lib.mem_simulation__free should use this lemma. *)
+Lemma mem_inj__free : forall mi Mem0 M2 Mem' mgb hi lo
+  (b2 : Values.block) (delta : Z) blk,
+  wf_sb_mi mgb mi Mem0 M2 ->
+  MoreMem.mem_inj mi Mem0 M2 ->
+  Mem.free Mem0 blk lo hi = ret Mem' ->
+  (lo, hi) = Mem.bounds Mem0 blk ->
+  mi blk = ret (b2, delta) ->
+  exists Mem2',
+    Mem.free M2 b2 (lo+delta) (hi+delta) = ret Mem2' /\
+    wf_sb_mi mgb mi Mem' Mem2' /\
+    MoreMem.mem_inj mi Mem' Mem2'.
+Proof.
+  intros mi Mem0 M2 Mem' mgb hi lo b2 delta blk Hwfmi Hmsim1 H0 HeqR2 H4.
+  assert ({ Mem2':Mem.mem | Mem.free M2 b2 (lo+delta) (hi+delta) = ret Mem2'}) 
+    as J.
+    apply Mem.range_perm_free.
+    apply Mem.free_range_perm in H0.
+    clear - H0 Hmsim1 H4.
+    unfold Mem.range_perm in *.
+    intros ofs J.
+    assert (lo <= ofs - delta < hi) as J'.
+      auto with zarith.
+    apply H0 in J'.
+    eapply MoreMem.perm_inj in J'; eauto.
+    assert (ofs - delta + delta = ofs) as EQ. auto with zarith.
+    rewrite EQ in J'. auto.
+  destruct J as [Mem2' J].
+  exists Mem2'. split; auto.
+  split.
+  SCase "wfmi".
+    clear - Hwfmi H0 J H4.
+    inversion_clear Hwfmi.
+    split; eauto with mem.
+    SSCase "Hmap3".
+      intros. erewrite Mem.nextblock_free in H; eauto.
+    SSCase "Hmap4".
+      intros. erewrite Mem.nextblock_free; eauto.
+    SSCase "bounds".
+      intros. apply mi_bounds in H. 
+      erewrite Mem.bounds_free; eauto.
+      erewrite Mem.bounds_free with (m2:=Mem2'); eauto.
+
+  SCase "msim".
+    clear - Hmsim1 Hwfmi H0 J H4.
+    inv Hwfmi.
+    eapply MoreMem.free_inj; eauto.
+Qed.
+
+Lemma mem_simulation__free : forall mi TD Mem1 Mem2 Mem1' Mem2'
+  ECs1 pinfo maxb lc1 F ptr1 ptr2
+  (Hmsim : mem_simulation pinfo maxb mi ((F, lc1) :: ECs1) Mem1 Mem2)
+  (Hsim: gv_inject mi ptr1 ptr2)
+  (Hmlc: free TD Mem1 ptr1 = ret Mem1')
+  (Hmlc': free TD Mem2 ptr2 = ret Mem2'),
+  mem_simulation pinfo maxb mi ((F, lc1) :: ECs1) Mem1' Mem2'.
+Proof.
+  intros.
+  destruct Hmsim as [J1 [J2 J3]].
+  apply free_inv in Hmlc.
+  apply free_inv in Hmlc'.
+  destruct Hmlc as [blk [ofs [hi [lo [H1 [H2 [H3 H4]]]]]]].
+  destruct Hmlc' as [blk' [ofs' [hi' [lo' [H1' [H2' [H3' H4']]]]]]].
+  unfold GV2ptr in *.
+  destruct ptr1 as [|[[]][]]; inv H1.
+  destruct ptr2 as [|[[]][]]; inv H1'.
+  inv Hsim. inv H1.
+  eapply mem_inj__free in H4; eauto.
+  destruct H4 as [Mem2'' [J4 [J5 J6]]].
+  assert (H6':=H6).
+  apply (mi_range_block maxb mi Mem1 Mem2 J3) in H6. subst.
+  apply (mi_bounds maxb mi Mem1 Mem2 J3) in H6'. 
+  rewrite H6' in H3. rewrite <- H3 in H3'. inv H3'.
+  assert (lo + 0 = lo) as EQ1. omega.
+  assert (hi + 0 = hi) as EQ2. omega.
+  rewrite EQ1 in J4. rewrite EQ2 in J4. clear EQ1 EQ2.
+  rewrite J4 in H4'. inv H4'.
+  split; auto.
+Qed.
+
+Lemma isnt_alloca_in_ECs_tail: forall pinfo (mi:MoreMem.meminj) EC1 EC2 ECs ,
+  (forall blk, 
+    ~ isnt_alloca_in_ECs pinfo (EC1 :: EC2 :: ECs) blk -> mi blk = merror) ->
+  (forall blk, 
+    ~ isnt_alloca_in_ECs pinfo (EC2 :: ECs) blk -> mi blk = merror).
+Proof.
+  intros.
+  apply H; auto. 
+  intro J. apply H0.
+  unfold isnt_alloca_in_ECs in J. unfold isnt_alloca_in_ECs.
+  intros.
+  apply J; auto.
+  simpl. simpl in Hin. destruct Hin; auto.
+Qed.
+
+Lemma mem_simulation_tail: forall pinfo mgb mi EC1 EC2 ECs M1 M2,
+  mem_simulation pinfo mgb mi (EC1 :: EC2 :: ECs) M1 M2 ->
+  mem_simulation pinfo mgb mi (EC2 :: ECs) M1 M2.
+Proof.
+  intros.
+  destruct H as [J1 [J2 J3]].
+  split; auto.
+  split; auto.
+    eapply isnt_alloca_in_ECs_tail; eauto.
+Qed.
+
+Ltac inv_mbind'' :=
+  repeat match goal with
+         | H : match ?e with
+               | Some _ => _
+               | None => None
+               end = Some _ |- _ => remember e as R; destruct R as [|]; inv H
+         | H : Some _ = match ?e with
+               | Some _ => _
+               | None => None
+               end |- _ => remember e as R; destruct R as [|]; inv H
+         | H :  ret _ = match ?p with
+                        | (_, _) => _
+                        end |- _ => destruct p
+         | H : if ?e then _ else False |- _ => 
+             remember e as R; destruct R; tinv H
+         | H : if ?e then False else _ |- _ => 
+             remember e as R; destruct R; tinv H
+         end.
+
+(* should move to MoreMem. *)
+Lemma free_left_nonmap_inj:
+  forall f m1 m2 b lo hi m1' (Hprop: f b = None),
+  MoreMem.mem_inj f m1 m2 ->
+  Mem.free m1 b lo hi = Some m1' ->
+  MoreMem.mem_inj f m1' m2.
+Proof.
+  intros. exploit Mem.free_result; eauto. intro FREE. inversion H. constructor.
+(* access *)
+  intros. eauto with mem. 
+(* mem_contents *)
+  intros. rewrite FREE; simpl.
+  assert (b=b1 /\ lo <= ofs < hi \/ (b<>b1 \/ ofs<lo \/ hi <= ofs)) 
+    by (unfold Values.block; omega).
+  destruct H3.
+    destruct H3. subst b1. uniq_result.
+
+    rewrite (Mem.clearN_out _ _ _ _ _ _ H3).
+    apply mi_memval; auto.
+    eapply Mem.perm_free_3; eauto.
+Qed.
+
+Lemma mem_inj__pfree : forall mi Mem0 M2 Mem' mgb hi lo
+  (b2 : Values.block) (delta : Z) blk,
+  wf_sb_mi mgb mi Mem0 M2 ->
+  MoreMem.mem_inj mi Mem0 M2 ->
+  Mem.free Mem0 blk lo hi = ret Mem' ->
+  (lo, hi) = Mem.bounds Mem0 blk ->
+  mi blk = None ->
+  wf_sb_mi mgb mi Mem' M2 /\ MoreMem.mem_inj mi Mem' M2.
+Proof.
+  intros mi Mem0 M2 Mem' mgb hi lo b2 delta blk Hwfmi Hmsim1 H0 HeqR2 H4.
+  split.
+  SCase "wfmi".
+    clear - Hwfmi H0 H4.
+    inversion_clear Hwfmi.
+    split; eauto with mem.
+    SSCase "Hmap3".
+      intros. erewrite Mem.nextblock_free in H; eauto.
+    SSCase "bounds".
+      intros. apply mi_bounds in H. 
+      erewrite Mem.bounds_free; eauto.
+
+  SCase "msim".
+    clear - Hmsim1 Hwfmi H0 H4.
+    inv Hwfmi.
+    eapply free_left_nonmap_inj; eauto.
+Qed.
+
+Lemma mem_simulation__pfree : forall mi TD Mem1 Mem2 Mem1' ECs1 pinfo maxb lc1
+  F (Hmsim : mem_simulation pinfo maxb mi ((F, lc1) :: ECs1) Mem1 Mem2)  
+  a (Hfree: free TD Mem1 (blk2GV TD a) = Some Mem1')
+  (Hinj: mi a = merror) (Hisallca: is_alloca_in_EC pinfo F lc1 a = true),
+  mem_simulation pinfo maxb mi ((F, lc1) :: ECs1) Mem1' Mem2.
+Proof.
+  intros.
+  destruct Hmsim as [J1 [J2 J3]].
+  apply free_inv in Hfree.
+  destruct Hfree as [blk [ofs [hi [lo [H1 [H2 [H3 H4]]]]]]].
+  unfold GV2ptr in *. unfold blk2GV, ptr2GV, val2GV in H1. inv H1. 
+  eapply mem_inj__pfree in H4; eauto.
+  destruct H4 as [H41 H42].
+  split; auto.
+Qed.
+
+Lemma mem_simulation__free_allocas : forall TD mgb F lc EC pinfo mi 
+  als1 M1 als2 M2 M1' 
+  (Hfree1: free_allocas TD M1 als1 = Some M1')
+  (Hmsim: mem_simulation pinfo mgb mi ((F,lc)::EC) M1 M2) M2'
+  (Halsim: als_simulation pinfo mi F lc als1 als2)
+  (Hfree2: free_allocas TD M2 als2 = Some M2'),
+  mem_simulation pinfo mgb mi ((F,lc)::EC) M1' M2'.
+Proof.
+  induction als1; destruct als2; simpl; intros.
+    uniq_result. auto.
+    uniq_result.
+
+    inv_mbind''. uniq_result.
+    destruct Halsim as [J1 J2].
+    eapply IHals1 with (M1:=m)(M2:=M2'); eauto.
+    eapply mem_simulation__pfree in Hmsim; eauto.
+
+    inv_mbind''. symmetry_ctx.
+    remember (is_alloca_in_EC pinfo F lc a) as R.
+    destruct R; destruct Halsim as [Halsim1 Halsim2].
+      eapply mem_simulation__pfree in Hmsim; eauto.
+      eapply IHals1 with (M1:=m1)(M2:=M2); eauto.
+      simpl. rewrite HeqR. auto.
+
+      eapply IHals1 with (M1:=m1)(M2:=m0); eauto.
+      eapply mem_simulation__free with (ptr1:=blk2GV TD a) (ptr2:=blk2GV TD m) 
+        in Hmsim; eauto.
+      unfold blk2GV, ptr2GV, val2GV. simpl.
+      constructor; auto.
+        assert (Int.repr 31 0 = Int.add 31 (Int.repr 31 0) (Int.repr 31 0)) 
+          as EQ.
+          rewrite Int.add_zero. auto.
+        rewrite EQ at 2.
+        econstructor; eauto.
+Qed.
+
+Lemma free_allocas_return_void_sim : forall TD mgb F lc F' lc' EC pinfo mi 
+  als1 M1 als2 M2 M1' 
+  (Hfree1: free_allocas TD M1 als1 = Some M1')
+  (Hmsim: mem_simulation pinfo mgb mi ((F,lc)::(F',lc')::EC) M1 M2) M2'
+  (Halsim: als_simulation pinfo mi F lc als1 als2)
+  (Hfree2: free_allocas TD M2 als2 = Some M2'),
+  mem_simulation pinfo mgb mi ((F',lc')::EC) M1' M2'.
+Proof.
+  intros.
+  eapply mem_simulation__free_allocas in Hmsim; eauto.
+  apply mem_simulation_tail in Hmsim; auto.
+Qed.
+
+Lemma is_alloca_in_EC_update_lc: forall pinfo F lc id0 gvs0 blk,
+  PI_f pinfo <> F \/ PI_id pinfo <> id0 ->
+  is_alloca_in_EC pinfo F lc blk =
+    is_alloca_in_EC pinfo F (updateAddAL (GVsT DGVs) lc id0 gvs0) blk.
+Proof.
+  intros.
+  unfold is_alloca_in_EC in *.
+  destruct (fdef_dec (PI_f pinfo) F); subst; auto.
+  destruct H as [H | H]; try congruence.
+  rewrite <- lookupAL_updateAddAL_neq; auto.
+Qed.  
+
+Lemma isnt_alloca_in_ECs_update_non_palloca : 
+  forall pinfo lc1 lc2 ECs F (mi:MoreMem.meminj) gvs3 id0,
+  PI_f pinfo <> F \/ PI_id pinfo <> id0 ->
+  updateAddAL (GVsT DGVs) lc1 id0 gvs3 = lc2 ->
+  (forall blk:mblock, 
+    ~ isnt_alloca_in_ECs pinfo ((F, lc1) :: strip_ECs ECs) blk -> 
+    mi blk = merror) ->
+  (forall blk:mblock, 
+    ~ isnt_alloca_in_ECs pinfo ((F, lc2) :: strip_ECs ECs) blk -> 
+    mi blk = merror).
+Proof.
+  intros. subst. 
+  apply H1. clear H1.
+  intro J. apply H2. clear H2.
+  unfold isnt_alloca_in_ECs in *.
+  intros.
+  simpl in Hin.
+  destruct Hin as [Hin | Hin]; subst.
+    inv Hin.
+    rewrite <- is_alloca_in_EC_update_lc; auto.
+    apply J. simpl. auto.
+
+    apply J. clear J. simpl. auto.
+Qed.
+
+Lemma mem_simulation__update_non_palloca : forall pinfo lc1 lc2 ECs F 
+  (mi:MoreMem.meminj) gvs3 id0 Mem1 Mem2 mgb,
+  PI_f pinfo <> F \/ PI_id pinfo <> id0 ->
+  updateAddAL (GVsT DGVs) lc1 id0 gvs3 = lc2 ->
+  mem_simulation pinfo mgb mi ((F, lc1) :: strip_ECs ECs) Mem1 Mem2 ->
+  mem_simulation pinfo mgb mi ((F, lc2) :: strip_ECs ECs) Mem1 Mem2.
+Proof.
+  intros.
+  destruct H1 as [J1 [J2 J3]].
+  repeat (split; auto);
+    eapply isnt_alloca_in_ECs_update_non_palloca; eauto; simpl; eauto.
+Qed.
+
+Lemma free_allocas_return_sim : forall TD mgb F 
+  Result lc F' i0 n c t v p lc' EC lc'' gl2 pinfo
+  (Hneq: PI_f pinfo <> F' \/ PI_id pinfo <> i0)
+  (Hupdate: Opsem.returnUpdateLocals TD (insn_call i0 n c t v p) Result lc lc' 
+              gl2 = ret lc'') mi
+  als M1 als2 M2 M1' M2'
+  (Hmsim: mem_simulation pinfo mgb mi ((F, lc) :: (F', lc') :: strip_ECs EC) 
+    M1 M2) 
+  (Hfree1: free_allocas TD M1 als = Some M1')
+  (Halsim: als_simulation pinfo mi F lc als als2)
+  (Hfree2: free_allocas TD M2 als2 = Some M2'),
+  mem_simulation pinfo mgb mi ((F',lc'') :: strip_ECs EC) M1' M2'.
+Proof.
+  intros.
+  eapply free_allocas_return_void_sim in Hmsim; eauto.
+  unfold Opsem.returnUpdateLocals in Hupdate.
+  inv_mbind'.
+  destruct n; inv H0; auto.
+  destruct t; inv H1; auto.
+  inv_mbind'.
+  eapply mem_simulation__update_non_palloca; eauto.
+Qed.
+
+Lemma als_simulation_update_lc: forall pinfo F lc mi id0 gvs0 als1 als2,
+  PI_f pinfo <> F \/ PI_id pinfo <> id0 ->
+  als_simulation pinfo mi F lc als1 als2 ->
+  als_simulation pinfo mi F (updateAddAL (GVsT DGVs) lc id0 gvs0) als1 als2.
+Proof.
+  induction als1; destruct als2; simpl; auto.
+    intros.
+    rewrite <- is_alloca_in_EC_update_lc; auto.
+    destruct (is_alloca_in_EC pinfo F lc a); auto.
+    destruct H0 as [J1 J2].
+    split; auto.
+
+    intros.
+    rewrite <- is_alloca_in_EC_update_lc; auto.
+    destruct (is_alloca_in_EC pinfo F lc a); destruct H0 as [J1 J2]; split; auto.
+Qed.
+
+Lemma returnUpdateLocals_als_simulation: forall pinfo mi F' lc' als' als3 TD i0 n
+  c t v p Result lc gl2 lc'' (Hsim: als_simulation pinfo mi F' lc' als' als3)
+  (Hprop: PI_f pinfo <> F' \/ PI_id pinfo <> i0)
+  (Hupdate: Opsem.returnUpdateLocals TD (insn_call i0 n c t v p) Result lc lc' 
+              gl2 = ret lc''),
+  als_simulation pinfo mi F' lc'' als' als3.
+Proof.
+  intros.
+  unfold Opsem.returnUpdateLocals in Hupdate.
+  inv_mbind'.
+  destruct n; inv H0; auto.
+  destruct t; inv H1; auto.
+  inv_mbind'.
+  apply als_simulation_update_lc; auto.
+Qed.
+  
+Lemma reg_simulation_update_non_palloca: forall pinfo F lc1 lc2 mi id0 gvs0 gvs3,
+  PI_f pinfo <> F \/ PI_id pinfo <> id0 ->
+  reg_simulation pinfo mi F lc1 lc2 ->
+  gv_inject mi gvs0 gvs3 ->
+  reg_simulation pinfo mi F (updateAddAL (GVsT DGVs) lc1 id0 gvs0)
+    (updateAddAL (GVsT DGVs) lc2 id0 gvs3).
+Proof.
+  unfold reg_simulation.
+  intros.
+  destruct (fdef_dec (PI_f pinfo) F); subst; intros.
+    assert (J:=@H0 i0). clear H0.
+    destruct H as [H | H]; try congruence.
+    destruct (id_dec (PI_id pinfo) i0); subst; auto.
+    destruct (id_dec id0 i0); subst.
+      rewrite lookupAL_updateAddAL_eq; auto.
+      rewrite lookupAL_updateAddAL_eq; auto.
+      intros. inv H2. inv H0. auto.
+
+      rewrite <- lookupAL_updateAddAL_neq; auto.
+      rewrite <- lookupAL_updateAddAL_neq; auto.
+
+    assert (J:=@H0 i0). clear H0.
+    destruct (id_dec id0 i0); subst.
+      rewrite lookupAL_updateAddAL_eq in H2; auto.
+      rewrite lookupAL_updateAddAL_eq in H3; auto.
+      inv H2. inv H3. auto.
+
+      rewrite <- lookupAL_updateAddAL_neq in H2; auto.
+      rewrite <- lookupAL_updateAddAL_neq in H3; auto.
+Qed.
+
+Lemma simulation__getOperandValue : forall pinfo maxb mi lc lc2 TD Mem Mem2 gl F 
+  v gv gv',
+  wf_globals maxb gl -> 
+  wf_sb_mi maxb mi Mem Mem2 ->
+  reg_simulation pinfo mi F lc lc2 ->
+  getOperandValue TD v lc gl = ret gv ->
+  getOperandValue TD v lc2 gl = ret gv' ->
+  gv_inject mi gv gv'.
+Proof.
+  intros.
+  unfold getOperandValue in *.
+  unfold reg_simulation in H1.
+  destruct (fdef_dec (PI_f pinfo) F); subst.
+    destruct v.
+(*
+(Hprop: PI_f pinfo <> F' \/ PI_id pinfo <> i0)
+    apply H1 in H2. auto.
+
+    exists gv. split; auto. eapply sb_mem_inj__const2GV; eauto.
+*)
+Admitted.
+
+(* from sb_ds_trans_lib, should go to sb_ds_gv_inject *)
+Lemma gv_inject__same_size : forall mi gv1 gv2,
+  gv_inject mi gv1 gv2 ->
+  sizeGenericValue gv1 = sizeGenericValue gv2.
+Proof.
+  intros mi gv1 gv2 Hinj.
+  induction Hinj; simpl; auto.
+Qed.
+
+Lemma simulation__lift_opt1: forall (mi : MoreMem.meminj) (TD : TargetData)
+  (t : typ) (g1 g2 g2' g1': GVsT DGVs)
+  (HeqR2 : lift_op1 DGVs (fit_gv TD t) g2 t = ret g2')
+  (HeqR1 : lift_op1 DGVs (fit_gv TD t) g1 t = ret g1')
+  (HeqR : gv_inject mi g1 g2),
+  gv_inject mi g1' g2'.
+Proof.
+  intros.
+Transparent lift_op1.
+  unfold lift_op1 in *. simpl in *.
+  unfold MDGVs.lift_op1 in *.
+  unfold fit_gv in *.
+  inv_mbind'. symmetry_ctx.
+  erewrite gv_inject__same_size in H0; eauto.
+  destruct (sizeGenericValue g2 =n= nat_of_Z (ZRdiv (Z_of_nat n) 8)).
+    inv HeqR2. inv H0. auto.
+
+    uniq_result.
+    eapply gv_inject_gundef; eauto.
+Opaque lift_op1.
+Qed.
+
+Lemma returnUpdateLocals_reg_simulation: forall pinfo mi F' lc' TD i0 n
+  c t v p Result lc gl lc'' lc3 lc''0 lc2 F Mem1 Mem2 maxb
+  (Hwfg: wf_globals maxb gl) (Hwfmi: wf_sb_mi maxb mi Mem1 Mem2)
+  (Hprop: PI_f pinfo <> F' \/ PI_id pinfo <> i0)
+  (Hsim: reg_simulation pinfo mi F' lc' lc3)
+  (Hsim': reg_simulation pinfo mi F lc lc2)
+  (Hupdate: Opsem.returnUpdateLocals TD (insn_call i0 n c t v p) Result lc lc' 
+              gl = ret lc'')
+  (Hupdate': Opsem.returnUpdateLocals TD (insn_call i0 n c t v p) Result lc2 lc3
+              gl = ret lc''0),
+  reg_simulation pinfo mi F' lc'' lc''0.
+Proof.
+  intros.
+  unfold Opsem.returnUpdateLocals in *.
+  inv_mbind'. symmetry_ctx.
+  eapply simulation__getOperandValue in HeqR; eauto.
+  destruct n; uniq_result; auto.
+  destruct t; tinv H0.
+  inv_mbind'. symmetry_ctx.
+  apply reg_simulation_update_non_palloca; auto.
+  eapply simulation__lift_opt1; eauto.
+Qed.
+
+Ltac destruct_ctx_other :=
+match goal with
+| Hwfpp : OpsemPP.wf_State
+            {|
+            OpsemAux.CurSystem := _;
+            OpsemAux.CurTargetData := ?TD;
+            OpsemAux.CurProducts := _;
+            OpsemAux.Globals := _;
+            OpsemAux.FunTable := _
+             |} _,
+  Hnoalias : Promotability.wf_State _ _ _ _,
+  Hsim : State_simulation _ _ _ _ _ ?Cfg2 ?St2 ,
+  Hop2 : Opsem.sInsn _ _ _ _ |- _ =>
+  destruct TD as [los nts];
+  destruct Hwfpp as 
+    [Hwfg [HwfSystem [HmInS [_ [
+     [Hreach1 [HBinF1 [HFinPs1 _]]] 
+     [ _ HwfCall'
+     ]]
+    ]]]]; subst;
+  destruct Cfg2 as [S2 TD2 Ps2 gl2 fs2];
+  destruct St2 as [ECs2 M2];
+  simpl in Hsim;
+  destruct Hsim as [EQ1 [Hpsim [Hstksim [EQ2 [EQ3 Hmsim]]]]]; subst;
+  destruct ECs2 as [|[F2 B2 cs2 tmn2 lc2 als2] ECs2]; tinv Hstksim;
+  destruct Hstksim as [Hecsim Hstksim];
+  unfold EC_simulation in Hecsim;
+  destruct Hecsim as 
+      [Hfsim2 [Heq1 [Halsim2 [Hbsim2 
+        [Heq3 [Heq4 [Hlcsim2 Hcssim2]]]]]]]; subst;
+  destruct Hnoalias as 
+    [
+      [[Hinscope' _] [HwfECs' HwfHT]] 
+      [[Hdisjals _] HwfM]
+    ]; simpl in Hdisjals;
+  fold Promotability.wf_ECStack in HwfECs'
+end.
+
+Lemma phis_simulation_inv: forall pinfo F ps1 ps2,
+  WF_PhiInfo pinfo -> uniqFdef F ->
+  phis_simulation pinfo F ps1 ps2 -> ps1 = ps2.
+Admitted.
+
+Lemma switchToNewBasicBlock_rsim : forall TD l1 l2 ps cs1 cs2 tmn1 tmn2 B1 B2
+  gl lc1 lc2 F pinfo mi lc1' lc2'
+  (H23 : @Opsem.switchToNewBasicBlock DGVs TD
+          (block_intro l1 ps cs1 tmn1) B1 gl lc1' = 
+         ret lc1)
+  (Hbsim2 : block_simulation pinfo F B1 B2)
+  (Hrsim: reg_simulation pinfo mi F lc1' lc2')
+  (H2 : Opsem.switchToNewBasicBlock TD
+         (block_intro l2 ps cs2 tmn2) B2 gl lc2' = 
+        ret lc2), reg_simulation pinfo mi F lc1 lc2.
+Admitted.
+
+Lemma switchToNewBasicBlock_asim: forall pinfo F l0 ps0 cs0 tmn0 als1 als2 lc 
+  lc' mi gl B TD,
+  WF_PhiInfo pinfo -> uniqFdef F ->
+  blockInFdefB (block_intro l0 ps0 cs0 tmn0) F = true ->
+  als_simulation pinfo mi F lc als1 als2 ->
+  Opsem.switchToNewBasicBlock TD (block_intro l0 ps0 cs0 tmn0) B gl lc = 
+    ret lc' ->
+  als_simulation pinfo mi F lc' als1 als2.
+Admitted.
+
+Lemma switchToNewBasicBlock_isnt_alloca_in_ECs : 
+  forall pinfo TD ECs F gl B B' blk lc1 lc2,
+  WF_PhiInfo pinfo -> uniqFdef F ->
+  blockInFdefB B' F = true ->
+  Opsem.switchToNewBasicBlock TD B' B gl lc1 = ret lc2 ->
+  isnt_alloca_in_ECs pinfo ((F,lc1) :: strip_ECs ECs) blk ->
+  isnt_alloca_in_ECs pinfo ((F,lc2) :: strip_ECs ECs) blk.
+Admitted.
+
+Lemma Promotability_wf_ECs__isnt_alloca_in_ECs: forall maxb pinfo TD M1 ECs1,
+  Promotability.wf_ECStack maxb pinfo TD M1 ECs1 ->
+  isnt_alloca_in_ECs pinfo (strip_ECs ECs1) (Mem.nextblock M1).
+Proof.
+  induction ECs1; simpl; intros.
+    unfold isnt_alloca_in_ECs.
+    intros. inv Hin.
+
+    destruct H as [H1 [H2 H3]].
+    unfold isnt_alloca_in_ECs in *.
+    intros.
+    simpl in Hin.
+    destruct Hin as [Hin | Hin]; subst.
+      inv Hin. destruct a. simpl in *.
+      destruct H1 as [H1 _].
+      unfold is_alloca_in_EC.
+      destruct (fdef_dec (PI_f pinfo) CurFunction); subst; auto.
+      remember (lookupAL (GVsT DGVs) Locals (PI_id pinfo)) as R.
+      destruct R as [[]|]; auto.
+      destruct p as [[]]; auto.
+      destruct l0; auto.
+      destruct (Z_eq_dec b (Mem.nextblock M1)); subst; auto.
+      symmetry in HeqR.
+      apply H1 in HeqR.
+      destruct HeqR as [HeqR _].
+      destruct HeqR as [HeqR _].
+      destruct HeqR as [mb [J1 [J2 J3]]].
+      rewrite Promotability.simpl_blk2GV in J1.
+      inv J1. 
+      contradict J3; omega.
+
+      apply IHECs1; simpl; auto.
+Qed.
+
+Lemma malloc__isnt_alloca_in_ECs: forall maxb pinfo TD Mem EC tsz0 gn align0 Mem'
+  mb (mi mi':MoreMem.meminj) (H1: Promotability.wf_ECStack maxb pinfo TD Mem EC)
+  (H2: malloc TD Mem tsz0 gn align0 = ret (Mem', mb))
+  (Hprop2 : forall b : mblock, b <> mb -> mi b = mi' b),
+  forall blk : mblock,
+    ~ isnt_alloca_in_ECs pinfo (strip_ECs EC) blk -> 
+    mi blk = merror -> mi' blk = merror.
+Proof.
+  intros.
+  destruct (zeq blk mb); subst.
+    apply MemProps.malloc_result in H2. subst.
+    contradict H.
+    eapply Promotability_wf_ECs__isnt_alloca_in_ECs; eauto.
+
+    rewrite <- Hprop2; auto.
+Qed.
+
+(*
+  lookupAL _ lc1 (PI_id pinfo) = None is important.
+
+  if p = alloca is in a loop, then at runtime, 
+    p can be assigned multiple times by p1, p2, p3...
+    all of which will be erased, and should not have corresponding memory block
+    in the transformed program.
+
+  But, we can only keep track of the last one, the earlier ones will be 
+   over-written...
+
+  In practice, a promotable allocation is always at the entry block, so
+  before its first assignment, its value must be none. Therefore, we are fine.
+*)
 Lemma als_simulation_weaken_palloca: 
   forall mi' mb mi pinfo lc1 ofs mc
   (Hlkup : lookupAL _ lc1 (PI_id pinfo) = None)
@@ -579,203 +1292,21 @@ Proof.
       contradict J. omega.
 Qed.
 
-Lemma reg_simulation_update_palloca: forall (pinfo : PhiInfo) 
-  (mi : MoreMem.meminj) TD (lc1 lc2 : Opsem.GVsMap)
-  (Hlcsim2 : reg_simulation pinfo mi (PI_f pinfo) lc1 lc2)
-  (mb : mblock) (mi' : MoreMem.meminj)
-  (Hinc : inject_incr mi mi'),
-  reg_simulation pinfo mi' (PI_f pinfo)
-    (updateAddAL (GVsT DGVs) lc1 (PI_id pinfo)
-       ($ blk2GV TD mb # typ_pointer (PI_typ pinfo) $)) lc2.
+Lemma dae_is_sim_removable_state: forall (maxb : Values.block) (pinfo : PhiInfo)
+  (mi : MoreMem.meminj) (Cfg1 : OpsemAux.Config) (St1 : Opsem.State) 
+  (Cfg2 : OpsemAux.Config) (St2 : Opsem.State) (Hwfpi : WF_PhiInfo pinfo)
+  (Hwfgl : wf_globals maxb (OpsemAux.Globals Cfg1)) (Hinbd : 0 <= maxb)
+  (Hnuse : used_in_fdef (PI_id pinfo) (PI_f pinfo) = false)
+  (Hwfpp : OpsemPP.wf_State Cfg1 St1)
+  (Hnoalias : Promotability.wf_State maxb pinfo Cfg1 St1)
+  (Hsim : State_simulation pinfo maxb mi Cfg1 St1 Cfg2 St2)
+  (Hrem : removable_State pinfo St1) (St1' : Opsem.State) (tr1 : trace)
+  (Hop1 : Opsem.sInsn Cfg1 St1 St1' tr1),
+  exists mi' : MoreMem.meminj,
+    State_simulation pinfo maxb mi' Cfg1 St1' Cfg2 St2 /\
+    tr1 = trace_nil /\ inject_incr mi mi'.
 Proof.
   intros.
-  unfold reg_simulation in *.
-  destruct (fdef_dec (PI_f pinfo) (PI_f pinfo)); try congruence.
-  intros.
-  assert (J:=@Hlcsim2 i0). clear Hlcsim2.
-  destruct (id_dec (PI_id pinfo) i0); subst; auto.
-  intros.
-  rewrite <- lookupAL_updateAddAL_neq in H; auto.
-  eapply J in H; eauto.
-  eapply gv_inject_incr; eauto.
-Qed.
-
-Lemma inject_incr__preserves__EC_simulation: forall pinfo mi mi' EC1 EC2,
-  EC_simulation pinfo mi EC1 EC2 ->
-  inject_incr mi mi' ->
-  EC_simulation pinfo mi' EC1 EC2.
-Admitted.
-
-Lemma inject_incr__preserves__ECs_simulation: forall pinfo mi mi' ECs1 ECs2,
-  ECs_simulation pinfo mi ECs1 ECs2 ->
-  inject_incr mi mi' ->
-  ECs_simulation pinfo mi' ECs1 ECs2.
-Proof.
-  induction ECs1; destruct ECs2; simpl; intros; auto.
-    destruct H as [H1 H2].
-    split; eauto using inject_incr__preserves__EC_simulation.
-Qed.
-
-Lemma inject_incr__preserves__ftable_simulation: forall mi mi' fs1 fs2,
-  ftable_simulation mi fs1 fs2 ->
-  inject_incr mi mi' ->
-  ftable_simulation mi' fs1 fs2.
-Admitted.
-
-Ltac destruct_ctx_return :=
-match goal with
-| Hwfpp : OpsemPP.wf_State
-            {|
-            OpsemAux.CurSystem := _;
-            OpsemAux.CurTargetData := ?TD;
-            OpsemAux.CurProducts := _;
-            OpsemAux.Globals := _;
-            OpsemAux.FunTable := _
-             |} _,
-  Hnoalias : Promotability.wf_State _ _ _ _,
-  Hsim : State_simulation _ _ _ _ _ ?Cfg2 ?St2 ,
-  Hop2 : Opsem.sInsn _ _ _ _ |- _ =>
-  destruct TD as [los nts];
-  destruct Hwfpp as 
-    [Hwfg [HwfSystem [HmInS [_ [
-     [Hreach1 [HBinF1 [HFinPs1 _]]] 
-     [ 
-       [
-         [Hreach2 [HBinF2 [HFinPs2 _]]]
-         _
-       ]
-       HwfCall'
-     ]]
-    ]]]]; subst;
-  destruct Cfg2 as [S2 TD2 Ps2 gl2 fs2];
-  destruct St2 as [ECs2 M2];
-  simpl in Hsim;
-  destruct Hsim as [EQ1 [Hpsim [Hstksim [EQ2 [EQ3 Hmsim]]]]]; subst;
-  destruct ECs2 as [|[F2 B2 cs2 tmn2 lc2 als2] ECs2]; tinv Hstksim;
-  destruct Hstksim as [Hecsim Hstksim];
-  destruct ECs2 as [|[F3 B3 cs3 tmn3 lc3 als3] ECs2]; tinv Hstksim;
-  destruct Hstksim as [Hecsim' Hstksim];
-  unfold EC_simulation in Hecsim;
-  destruct Hecsim as 
-      [Hfsim2 [Heq1 [Halsim2 [Hbsim2 
-        [Heq3 [Heq4 [Hlcsim2 Hcssim2]]]]]]]; subst;
-  destruct Hecsim' as 
-      [Hfsim2' [Heq1' [Halsim2' [Hbsim2' 
-        [Heq3' [Heq4' [Hlcsim2' Hcssim2']]]]]]]; subst;
-  destruct Hnoalias as 
-    [
-      [[Hinscope1' _] [[[Hinscope2' _] [HwfECs' _]] _]] 
-      [[Hdisjals _] HwfM]
-    ]; simpl in Hdisjals;
-  fold Promotability.wf_ECStack in HwfECs';
-  apply cmds_simulation_nil_inv in Hcssim2; subst;
-  wfCall_inv
-end.
-
-
-Lemma free_allocas_return_sim : forall TD mgb als M1 als2 M2 M1' F l3 ps3 cs0 rid
-  RetTy Result lc F' B' i0 n c t v p cs' tmn3 lc' als' EC lc'' gl2 pinfo
-  (Hupdate: Opsem.returnUpdateLocals TD (insn_call i0 n c t v p) Result lc lc' 
-              gl2 = ret lc'') mi
-  (Hfree1: free_allocas TD M1 als = Some M1')
-  (Hmsim: Mem_simulation pinfo mgb mi
-    ({| Opsem.CurFunction := F;
-        Opsem.CurBB := block_intro l3 ps3 (cs0 ++ nil)
-                              (insn_return rid RetTy Result);
-        Opsem.CurCmds := nil;
-        Opsem.Terminator := insn_return rid RetTy Result;
-        Opsem.Locals := lc;
-        Opsem.Allocas := als |}
-             :: {|
-                Opsem.CurFunction := F';
-                Opsem.CurBB := B';
-                Opsem.CurCmds := insn_call i0 n c t v p :: cs';
-                Opsem.Terminator := tmn3;
-                Opsem.Locals := lc';
-                Opsem.Allocas := als' |} :: EC) M1 M2) M2'
-  (Halsim: als_simulation pinfo mi F lc als als2)
-  (Hfree2: free_allocas TD M2 als2 = Some M2'),
-  Mem_simulation pinfo mgb mi 
-    ({| Opsem.CurFunction := F';
-        Opsem.CurBB := B';
-        Opsem.CurCmds := cs';
-        Opsem.Terminator := tmn3;
-        Opsem.Locals := lc'';
-        Opsem.Allocas := als' |} :: EC) M1' M2'.
-Admitted.
-
-Lemma returnUpdateLocals_als_simulation: forall pinfo mi F' lc' als' als3 TD i0 n
-  c t v p Result lc gl2 lc'' (Hsim: als_simulation pinfo mi F' lc' als' als3)
-  (Hupdate: Opsem.returnUpdateLocals TD (insn_call i0 n c t v p) Result lc lc' 
-              gl2 = ret lc''),
-  als_simulation pinfo mi F' lc'' als' als3.
-Admitted.
-  
-Lemma returnUpdateLocals_reg_simulation: forall pinfo mi F' lc' TD i0 n
-  c t v p Result lc gl2 lc'' lc3 lc''0 lc2 F
-  (Hsim: reg_simulation pinfo mi F' lc' lc3)
-  (Hsim': reg_simulation pinfo mi F lc lc2)
-  (Hupdate: Opsem.returnUpdateLocals TD (insn_call i0 n c t v p) Result lc lc' 
-              gl2 = ret lc'')
-  (Hupdate': Opsem.returnUpdateLocals TD (insn_call i0 n c t v p) Result lc2 lc3
-              gl2 = ret lc''0),
-  reg_simulation pinfo mi F' lc'' lc''0.
-Admitted.
-
-Lemma free_allocas_return_void_sim : forall TD mgb als M1 als2 M2 M1' F l3 ps3 
-  cs0 rid lc F' B' i0 n c t v p cs' tmn3 lc' als' EC pinfo mi
-  (Hfree1: free_allocas TD M1 als = Some M1')
-  (Hmsim: Mem_simulation pinfo mgb mi
-    ({| Opsem.CurFunction := F;
-        Opsem.CurBB := block_intro l3 ps3 (cs0 ++ nil) (insn_return_void rid);
-        Opsem.CurCmds := nil;
-        Opsem.Terminator := insn_return_void rid;
-        Opsem.Locals := lc;
-        Opsem.Allocas := als |}
-             :: {|
-                Opsem.CurFunction := F';
-                Opsem.CurBB := B';
-                Opsem.CurCmds := insn_call i0 n c t v p :: cs';
-                Opsem.Terminator := tmn3;
-                Opsem.Locals := lc';
-                Opsem.Allocas := als' |} :: EC) M1 M2) M2'
-  (Halsim: als_simulation pinfo mi F lc als als2)
-  (Hfree2: free_allocas TD M2 als2 = Some M2'),
-  Mem_simulation pinfo mgb mi 
-    ({| Opsem.CurFunction := F';
-        Opsem.CurBB := B';
-        Opsem.CurCmds := cs';
-        Opsem.Terminator := tmn3;
-        Opsem.Locals := lc';
-        Opsem.Allocas := als' |} :: EC) M1' M2'.
-Admitted.
-
-Lemma dae_is_sim : forall maxb pinfo mi Cfg1 St1 Cfg2 St2
-  (Hwfpi: WF_PhiInfo pinfo) 
-  (Hwfgl: sb_ds_gv_inject.wf_globals maxb (OpsemAux.Globals Cfg1)) 
-  (Hinbd: 0 <= maxb) (Hnuse: used_in_fdef (PI_id pinfo) (PI_f pinfo) = false)
-  (Hwfpp: OpsemPP.wf_State Cfg1 St1) 
-  (Hnoalias: Promotability.wf_State maxb pinfo Cfg1 St1) 
-  (Hsim: State_simulation pinfo maxb mi Cfg1 St1 Cfg2 St2),
-  (forall (Hrem: removable_State pinfo St1) St1' tr1 
-     (Hop1: Opsem.sInsn Cfg1 St1 St1' tr1), 
-     exists mi',
-       State_simulation pinfo maxb mi' Cfg1 St1' Cfg2 St2 /\ tr1 = trace_nil /\
-       Values.inject_incr mi mi') /\
-  (forall (Hnrem: ~removable_State pinfo St1) St1' St2' tr1 tr2
-     (Hop2: Opsem.sInsn Cfg2 St2 St2' tr2) 
-     (Hop1: Opsem.sInsn Cfg1 St1 St1' tr1), 
-     exists mi',
-       State_simulation pinfo maxb mi' Cfg1 St1' Cfg2 St2' /\ tr1 = tr2 /\
-       Values.inject_incr mi mi').
-Proof.
-
-Local Opaque inscope_of_tmn inscope_of_cmd.
-
-  intros.
-  split; intros.
-Case "removable state".
-  
   destruct Cfg1 as [S1 [los nts] Ps1 gl1 fs1].
   destruct St1 as [ECs1 M1].
   destruct ECs1 as [|[F1 B1 [|c1 cs1] tmn1 lc1 als1] ECs1]; tinv Hrem.
@@ -822,12 +1353,458 @@ Case "removable state".
   repeat_solve.
     eapply als_simulation_update_palloca; eauto.
       admit. (*dom*)
-        eapply reg_simulation_update_palloca; eauto.
+    eapply reg_simulation_update_palloca; eauto.
     eapply cmds_simulation_elim_cons_inv; eauto.
     eapply inject_incr__preserves__ECs_simulation; eauto.
+      eapply malloc__isnt_alloca_in_ECs; eauto.
     eapply inject_incr__preserves__ftable_simulation; eauto.
+Qed.
+
+Lemma not_removable_State_inv: forall pinfo St,
+  ~ removable_State pinfo St ->
+  match St with 
+  | {| Opsem.ECS := {| Opsem.CurFunction := F;
+                       Opsem.CurBB := _;
+                       Opsem.CurCmds := c :: _;
+                       Opsem.Terminator := _;
+                       Opsem.Locals := _;
+                       Opsem.Allocas := _ |} :: _;
+       Opsem.Mem := Mem |} => PI_f pinfo <> F \/ PI_id pinfo <> getCmdLoc c
+  | _ => True
+  end.
+Proof.
+  intros.
+  destruct St; auto.
+  destruct ECS; auto.
+  destruct e; auto.
+  destruct CurCmds; auto.
+  simpl in H.
+  destruct (fdef_dec (PI_f pinfo) CurFunction); subst; auto.
+  destruct (id_dec (PI_id pinfo) (getCmdLoc c)); subst; auto.
+Qed.
+
+Lemma simulation__BOP : forall maxb mi lc lc2 TD gl F bop0 sz0 
+    v1 v2 gv3 gv3' pinfo Mem Mem2,
+  wf_globals maxb gl -> 
+  wf_sb_mi maxb mi Mem Mem2 ->
+  reg_simulation pinfo mi F lc lc2 ->
+  BOP TD lc gl bop0 sz0 v1 v2 = ret gv3 ->
+  BOP TD lc2 gl bop0 sz0 v1 v2 = ret gv3' ->
+  gv_inject mi gv3 gv3'.
+Proof.  
+  intros maxb mi lc lc2 TD gl F bop0 sz0 v1 v2 gv3 gv3' pinfo Me Mem2 Hwfg H0 H1 
+    H2 H3.
+  unfold BOP in *.
+  inv_mbind'. symmetry_ctx.
+  eapply simulation__getOperandValue with (lc2:=lc2) in HeqR1; eauto.
+  eapply simulation__getOperandValue with (lc2:=lc2) in HeqR2; eauto.
+  eapply simulation__mbop in H2; eauto.
+  destruct H2 as [gv4 [J1 J2]].
+  uniq_result. auto.
+Qed.
+
+Lemma simulation__FBOP : forall maxb mi lc lc2 TD gl F fop0 fp
+    v1 v2 gv3 gv3' pinfo Mem Mem2,
+  wf_globals maxb gl -> 
+  wf_sb_mi maxb mi Mem Mem2 ->
+  reg_simulation pinfo mi F lc lc2 ->
+  FBOP TD lc gl fop0 fp v1 v2 = ret gv3 ->
+  FBOP TD lc2 gl fop0 fp v1 v2 = ret gv3' ->
+  gv_inject mi gv3 gv3'.
+Proof.  
+  intros maxb mi lc lc2 TD gl F fop0 fp v1 v2 gv3 gv3' pinfo Me Mem2 Hwfg H0 H1 
+    H2 H3.
+  unfold FBOP in *.
+  inv_mbind'. symmetry_ctx.
+  eapply simulation__getOperandValue with (lc2:=lc2) in HeqR1; eauto.
+  eapply simulation__getOperandValue with (lc2:=lc2) in HeqR2; eauto.
+  eapply simulation__mfbop in H2; eauto.
+  destruct H2 as [gv4 [J1 J2]].
+  uniq_result. auto.
+Qed.
+
+Lemma simulation__ExtractValue : forall mi gv1 gv1' TD t1 l0 gv gv' gl2 lc
+  lc2 v F pinfo Mem Mem2 maxb,
+  wf_globals maxb gl2 -> 
+  wf_sb_mi maxb mi Mem Mem2 ->
+  reg_simulation pinfo mi F lc lc2 ->
+  getOperandValue TD v lc gl2 = Some gv1 ->
+  getOperandValue TD v lc2 gl2 = Some gv1' ->
+  extractGenericValue TD t1 gv1 l0 = Some gv ->
+  extractGenericValue TD t1 gv1' l0 = Some gv' ->
+  gv_inject mi gv gv'.
+Proof.
+  intros.
+  eapply simulation__getOperandValue with (lc2:=lc2) in H2; eauto.
+  eapply simulation__extractGenericValue in H4; eauto.
+  destruct H4 as [gv'' [J1 J2]].
+  uniq_result. auto.
+Qed.
+
+Lemma simulation__InsertValue : forall mi gv1 gv1' TD t1 l0 gv2 gv2' gl2 lc
+  lc2 v1 v2 F pinfo Mem Mem2 maxb gv3 gv3' t2,
+  wf_globals maxb gl2 -> 
+  wf_sb_mi maxb mi Mem Mem2 ->
+  reg_simulation pinfo mi F lc lc2 ->
+  getOperandValue TD v1 lc gl2 = Some gv1 ->
+  getOperandValue TD v1 lc2 gl2 = Some gv1' ->
+  getOperandValue TD v2 lc gl2 = Some gv2 ->
+  getOperandValue TD v2 lc2 gl2 = Some gv2' ->
+  insertGenericValue TD t1 gv1 l0 t2 gv2 = ret gv3 ->
+  insertGenericValue TD t1 gv1' l0 t2 gv2' = ret gv3' ->
+  gv_inject mi gv3 gv3'.
+Proof.
+  intros.
+  eapply simulation__getOperandValue with (lc2:=lc2) in H2; eauto.
+  eapply simulation__getOperandValue with (lc2:=lc2) in H4; eauto.
+  eapply simulation__insertGenericValue in H6; eauto.
+  destruct H6 as [gv'' [J1 J2]].
+  uniq_result. auto.
+Qed.
+
+Lemma simulation__values2GVs : forall maxb mi lc lc2 TD Mem Mem2 gl F idxs gvs 
+  gvs' pinfo,
+  wf_globals maxb gl -> 
+  wf_sb_mi maxb mi Mem Mem2 ->
+  reg_simulation pinfo mi F lc lc2 ->
+  values2GVs TD idxs lc gl = ret gvs ->
+  values2GVs TD idxs lc2 gl = ret gvs' ->
+  gvs_inject mi gvs gvs'.
+Proof.
+  induction idxs; simpl; intros.
+    inv H2. inv H3. simpl. auto.
+
+    inv_mbind'. symmetry_ctx.
+    eapply simulation__getOperandValue with (lc2:=lc2) in HeqR1; eauto.
+    simpl. split; eauto.
+Qed.
+
+Lemma simulation__GEP : forall maxb mi TD Mem Mem2 inbounds0 vidxs1 vidxs2 gv1 
+    gv1' gv2 gv2' t gl2 lc lc2 idxs v F pinfo,
+  wf_globals maxb gl2 -> 
+  wf_sb_mi maxb mi Mem Mem2 ->
+  reg_simulation pinfo mi F lc lc2 ->
+  getOperandValue TD v lc gl2 = Some gv1 ->
+  getOperandValue TD v lc2 gl2 = Some gv1' ->
+  values2GVs TD idxs lc gl2 = Some vidxs1 ->
+  values2GVs TD idxs lc2 gl2 = Some vidxs2 ->
+  GEP TD t gv1 vidxs1 inbounds0 = ret gv2 ->
+  GEP TD t gv1' vidxs2 inbounds0 = ret gv2' ->
+  gv_inject mi gv2 gv2'.
+Proof.
+  intros.
+  eapply simulation__getOperandValue with (lc2:=lc2) in H2; eauto.
+  eapply simulation__values2GVs with (lc2:=lc2) in H4; eauto.
+  eapply sb_ds_gv_inject.simulation__GEP in H6; eauto.
+  destruct H6 as [gv'' [J1 J2]].
+  uniq_result. auto.
+Qed.
+
+Lemma simulation__TRUNC : forall maxb mi lc lc2 TD gl F op t1 t2
+    v1 gv3 gv3' pinfo Mem Mem2,
+  wf_globals maxb gl -> 
+  wf_sb_mi maxb mi Mem Mem2 ->
+  reg_simulation pinfo mi F lc lc2 ->
+  TRUNC TD lc gl op t1 v1 t2 = ret gv3 ->
+  TRUNC TD lc2 gl op t1 v1 t2 = ret gv3' ->
+  gv_inject mi gv3 gv3'.
+Proof.  
+  intros maxb mi lc lc2 TD gl F op t1 t2 v1 gv3 gv3' pinfo Mem Mem2 Hwfg H0 H1 
+    H2 H3.
+  unfold TRUNC in *.
+  inv_mbind'. symmetry_ctx.
+  eapply simulation__getOperandValue with (lc2:=lc2) in HeqR; eauto.
+  eapply simulation__mtrunc in H3; eauto.
+  destruct H3 as [gv4 [J1 J2]].
+  uniq_result. auto.
+Qed.
+
+Lemma simulation__EXT : forall maxb mi lc lc2 TD gl F op t1 t2
+    v1 gv3 gv3' pinfo Mem Mem2,
+  wf_globals maxb gl -> 
+  wf_sb_mi maxb mi Mem Mem2 ->
+  reg_simulation pinfo mi F lc lc2 ->
+  EXT TD lc gl op t1 v1 t2 = ret gv3 ->
+  EXT TD lc2 gl op t1 v1 t2 = ret gv3' ->
+  gv_inject mi gv3 gv3'.
+Proof.  
+  intros maxb mi lc lc2 TD gl F op t1 t2 v1 gv3 gv3' pinfo Mem Mem2 Hwfg H0 H1 
+    H2 H3.
+  unfold EXT in *.
+  inv_mbind'. symmetry_ctx.
+  eapply simulation__getOperandValue with (lc2:=lc2) in HeqR; eauto.
+  eapply simulation__mext in H3; eauto.
+  destruct H3 as [gv4 [J1 J2]].
+  uniq_result. auto.
+Qed.
+
+Lemma simulation__CAST : forall maxb mi lc lc2 TD gl F op t1 t2
+    v1 gv3 gv3' pinfo Mem Mem2,
+  wf_globals maxb gl -> 
+  wf_sb_mi maxb mi Mem Mem2 ->
+  reg_simulation pinfo mi F lc lc2 ->
+  CAST TD lc gl op t1 v1 t2 = ret gv3 ->
+  CAST TD lc2 gl op t1 v1 t2 = ret gv3' ->
+  gv_inject mi gv3 gv3'.
+Proof.  
+  intros maxb mi lc lc2 TD gl F op t1 t2 v1 gv3 gv3' pinfo Mem Mem2 Hwfg H0 H1 
+    H2 H3.
+  unfold CAST in *.
+  inv_mbind'. symmetry_ctx.
+  eapply simulation__getOperandValue with (lc2:=lc2) in HeqR; eauto.
+  eapply simulation__mcast in H3; eauto.
+  destruct H3 as [gv4 [J1 J2]].
+  uniq_result. auto.
+Qed.
+
+Lemma simulation__ICMP : forall maxb mi lc lc2 TD gl F cond0 t1 v1 v2 gv3 gv3' 
+  pinfo Mem Mem2, 
+  wf_globals maxb gl -> 
+  wf_sb_mi maxb mi Mem Mem2 ->
+  reg_simulation pinfo mi F lc lc2 ->
+  ICMP TD lc gl cond0 t1 v1 v2 = ret gv3 ->
+  ICMP TD lc2 gl cond0 t1 v1 v2 = ret gv3' ->
+  gv_inject mi gv3 gv3'.
+Proof.  
+  intros maxb mi lc lc2 TD gl F cond0 t1 v1 v2 gv3 gv3' pinfo Me Mem2 Hwfg H0 H1 
+    H2 H3.
+  unfold ICMP in *.
+  inv_mbind'. symmetry_ctx.
+  eapply simulation__getOperandValue with (lc2:=lc2) in HeqR1; eauto.
+  eapply simulation__getOperandValue with (lc2:=lc2) in HeqR2; eauto.
+  eapply simulation__micmp in H2; eauto.
+  destruct H2 as [gv4 [J1 J2]].
+  uniq_result. auto.
+Qed.
+
+Lemma simulation__FCMP : forall maxb mi lc lc2 TD gl F fcond0 fp v1 v2 gv3 gv3' 
+  pinfo Mem Mem2, 
+  wf_globals maxb gl -> 
+  wf_sb_mi maxb mi Mem Mem2 ->
+  reg_simulation pinfo mi F lc lc2 ->
+  FCMP TD lc gl fcond0 fp v1 v2 = ret gv3 ->
+  FCMP TD lc2 gl fcond0 fp v1 v2 = ret gv3' ->
+  gv_inject mi gv3 gv3'.
+Proof.  
+  intros maxb mi lc lc2 TD gl F cond0 t1 v1 v2 gv3 gv3' pinfo Me Mem2 Hwfg H0 H1 
+    H2 H3.
+  unfold FCMP in *.
+  inv_mbind'. symmetry_ctx.
+  eapply simulation__getOperandValue with (lc2:=lc2) in HeqR1; eauto.
+  eapply simulation__getOperandValue with (lc2:=lc2) in HeqR2; eauto.
+  eapply simulation__mfcmp in H2; eauto.
+  destruct H2 as [gv4 [J1 J2]].
+  uniq_result. auto.
+Qed.
+
+Lemma mem_simulation__wf_sb_sim: forall pinfo maxb mi ECs M1 M2,
+  mem_simulation pinfo maxb mi ECs M1 M2 -> wf_sb_mi maxb mi M1 M2.  
+Proof.
+  intros. destruct H as [_ [_ H]]; auto.
+Qed.
+
+Ltac dse_is_sim_common_case :=
+match goal with
+| Hcssim2: cmds_simulation _ _ _ _,
+  Hop2: Opsem.sInsn _ _ _ _,
+  Hmsim: mem_simulation _ _ ?mi _ _ _ |- _ =>
+  apply cmds_simulation_nelim_cons_inv in Hcssim2; simpl; auto;
+  destruct Hcssim2 as [cs3' [Heq Hcssim2]]; subst;
+  inv Hop2; uniq_result;
+  exists mi;
+  repeat_solve; try solve [
+    apply als_simulation_update_lc; auto |
+    apply reg_simulation_update_non_palloca; eauto using 
+      simulation__BOP, simulation__FBOP, simulation__ExtractValue,
+      simulation__InsertValue, simulation__GEP, simulation__TRUNC,
+      simulation__EXT, simulation__ICMP, simulation__FCMP, simulation__CAST,
+      mem_simulation__wf_sb_sim |
+    eapply mem_simulation__update_non_palloca; eauto; simpl; eauto
+  ]
+end.
+
+Lemma mem_simulation__malloc : forall mi TD Mem1 Mem2 tsz gn Mem1' Mem2' mb1
+  mb2 v ECs1 pinfo maxb lc1 t id0 align0 F gn'
+  (Hnrem : PI_f pinfo <> F \/
+          PI_id pinfo <> getCmdLoc (insn_malloc id0 t v align0))
+  (Hmsim : mem_simulation pinfo maxb mi ((F,lc1) :: ECs1) Mem1 Mem2)
+  (Hsim: gv_inject mi gn gn')
+  (Hmlc: malloc TD Mem1 tsz gn align0 = ret (Mem1', mb1))
+  (Hmlc': malloc TD Mem2 tsz gn' align0 = ret (Mem2', mb2)),
+  exists mi',
+    mem_simulation pinfo maxb mi'
+            ((F,updateAddAL (GVsT DGVs) lc1 id0
+                 ($ blk2GV TD mb1 # typ_pointer t $)) :: ECs1) Mem1' Mem2' /\
+    Values.inject_incr mi mi' /\
+    mi' mb1 = Some (mb2, 0) /\
+    (forall b, b <> mb1 -> mi b = mi' b).
+Admitted.
+
+Lemma als_simulation___malloc: forall pinfo F als1 als2 lc mi id0 mi' mb mb0 TD 
+  t (Hprop1 : mi' mb = ret (mb0, 0))
+  (Hprop2 : forall b : mblock, b <> mb -> mi b = mi' b),
+  PI_f pinfo <> F \/ PI_id pinfo <> id0 ->
+  als_simulation pinfo mi F lc als1 als2 ->
+  als_simulation pinfo mi' F 
+    (updateAddAL (GVsT DGVs) lc id0 ($ blk2GV TD mb # typ_pointer t $)) 
+    als1 als2.
+Admitted.
+
+Lemma reg_simulation___malloc: forall pinfo F lc1 lc2 mi id0 mi' mb1 mb2 TD 
+  t (Hprop1 : mi' mb1 = ret (mb2, 0))
+  (Hprop2 : forall b : mblock, b <> mb1 -> mi b = mi' b),
+  PI_f pinfo <> F \/ PI_id pinfo <> id0 ->
+  reg_simulation pinfo mi F lc1 lc2 ->
+  reg_simulation pinfo mi' F
+    (updateAddAL (GVsT DGVs) lc1 id0 ($ blk2GV TD mb1 # typ_pointer t $))
+    (updateAddAL (GVsT DGVs) lc2 id0 ($ blk2GV TD mb2 # typ_pointer t $)).
+Admitted.
+
+Lemma mem_simulation__alloca : forall mi TD Mem1 Mem2 tsz gn Mem1' Mem2' mb1
+  mb2 ECs1 pinfo maxb lc1 t id0 align0 F gn'
+  (Hnrem : PI_f pinfo <> F \/ PI_id pinfo <> id0)
+  (Hmsim : mem_simulation pinfo maxb mi ((F,lc1) :: ECs1) Mem1 Mem2)
+  (Hsim: gv_inject mi gn gn')
+  (Hmlc: malloc TD Mem1 tsz gn align0 = ret (Mem1', mb1))
+  (Hmlc': malloc TD Mem2 tsz gn' align0 = ret (Mem2', mb2)),
+  exists mi',
+    mem_simulation pinfo maxb mi'
+            ((F, updateAddAL (GVsT DGVs) lc1 id0
+                   ($ blk2GV TD mb1 # typ_pointer t $)) :: ECs1) Mem1' Mem2' /\
+    Values.inject_incr mi mi' /\
+    mi' mb1 = Some (mb2, 0) /\
+    (forall b, b <> mb1 -> mi b = mi' b).
+Admitted.
+
+Lemma als_simulation___alloca: forall pinfo F als1 als2 lc mi id0 mi' mb mb0 TD 
+  t (Hprop1 : mi' mb = ret (mb0, 0))
+  (Hprop2 : forall b : mblock, b <> mb -> mi b = mi' b),
+  PI_f pinfo <> F \/ PI_id pinfo <> id0 ->
+  als_simulation pinfo mi F lc als1 als2 ->
+  als_simulation pinfo mi' F 
+    (updateAddAL (GVsT DGVs) lc id0 ($ blk2GV TD mb # typ_pointer t $)) 
+    (mb::als1) (mb0::als2).
+Admitted.
+
+Lemma simulation__mload : forall mi TD pinfo maxb Mem1 Mem2 gvp1 align0 gv1 gv2 t
+  gvp2 st,  
+  mem_simulation pinfo maxb mi st Mem1 Mem2 ->
+  mload TD Mem1 gvp1 t align0 = ret gv1 ->
+  mload TD Mem2 gvp2 t align0 = ret gv2 ->
+  gv_inject mi gvp1 gvp2 ->
+  gv_inject mi gv1 gv2.
+Admitted.
+
+Lemma simulation__mstore : forall mi TD pinfo Mem1 Mem2 gvp1 gv1 gvp2 
+  gv2 Mem1' Mem2' maxb F t align0 lc ECs,
+  mem_simulation pinfo maxb mi ((F,lc) :: strip_ECs ECs) Mem1 Mem2 ->
+  mstore TD Mem1 gvp1 t gv1 align0 = ret Mem1' ->
+  mstore TD Mem2 gvp2 t gv2 align0 = ret Mem2' ->
+  gv_inject mi gvp1 gvp2 ->
+  gv_inject mi gv1 gv2 ->
+  mem_simulation pinfo maxb mi ((F, lc) :: strip_ECs ECs) Mem1' Mem2'.
+Admitted.
+
+Lemma lookupFdefViaPtr__simulation : forall pinfo Ps1 Ps2 fptr1 fptr2 f1 f2 fs1
+  fs2 mi,
+  ftable_simulation mi fs1 fs2 ->
+  OpsemAux.lookupFdefViaPtr Ps2 fs2 fptr2 = Some f2 ->
+  products_simulation pinfo Ps1 Ps2 ->
+  gv_inject mi fptr1 fptr2 ->
+  OpsemAux.lookupFdefViaPtr Ps1 fs1 fptr1 = Some f1 ->
+  fdef_simulation pinfo f1 f2.
+Proof.
+  intros.
+  unfold OpsemAux.lookupFdefViaPtr in *.
+  remember (OpsemAux.lookupFdefViaGVFromFunTable fs1 fptr1) as R1.
+  destruct R1 as [fid1|]; inv H3. 
+  remember (OpsemAux.lookupFdefViaGVFromFunTable fs2 fptr2) as R2.
+  destruct R2 as [fid2|]; inv H0. 
+  eapply products_simulation__fdef_simulation; eauto.
+Admitted.
+
+Lemma reg_simulation__initLocals: forall pinfo mi F lc1 lc2 lp gl gvs1 gvs2 lc1'
+  lc2' la TD fa0 rt0 fid0 va0 lb,
+  reg_simulation pinfo mi F lc1 lc2 ->
+  Opsem.params2GVs TD lp lc1 gl = ret gvs1 ->
+  Opsem.params2GVs TD lp lc2 gl = ret gvs2 ->
+  Opsem.initLocals TD la gvs1 = ret lc1' ->
+  Opsem.initLocals TD la gvs2 = ret lc2' ->
+  reg_simulation pinfo mi 
+    (fdef_intro (fheader_intro fa0 rt0 fid0 la va0) lb) lc1' lc2'.
+Admitted.
+
+Lemma lookupFdefViaPtr__simulation_l2r : forall pinfo Ps1 Ps2 fptr1 fptr2 f1 
+  fs1 fs2 mi,
+  products_simulation pinfo Ps1 Ps2 ->
+  ftable_simulation mi fs1 fs2 ->
+  gv_inject mi fptr1 fptr2 ->
+  OpsemAux.lookupFdefViaPtr Ps1 fs1 fptr1 = Some f1 ->
+  exists f2, 
+    OpsemAux.lookupFdefViaPtr Ps2 fs2 fptr2 = Some f2 /\
+    fdef_simulation pinfo f1 f2.
+Admitted.
+
+Lemma lookupExFdecViaPtr__simulation_l2r : forall pinfo Ps1 Ps2 fptr1 fptr2 f fs1
+  fs2 mi,
+  products_simulation pinfo Ps1 Ps2 ->
+  ftable_simulation mi fs1 fs2 ->
+  gv_inject mi fptr1 fptr2 ->
+  OpsemAux.lookupExFdecViaPtr Ps1 fs1 fptr1 = Some f ->
+  OpsemAux.lookupExFdecViaPtr Ps2 fs2 fptr2 = Some f.
+Admitted.
+
+Lemma callExternalFunction__mem_simulation: forall pinfo mi M1 M2 fid0 gvs1 
+  gvs2 oresult1 M1' oresult2 M2' mgb gl lc1 lc2 TD F rid noret0 ft lp
+  EC lc1' lc2' als1 als2,
+  mem_simulation pinfo mgb mi ((F,lc1) :: strip_ECs EC) M1 M2 ->
+  reg_simulation pinfo mi F lc1 lc2 ->
+  Opsem.params2GVs TD lp lc1 gl = ret gvs1 ->
+  Opsem.params2GVs TD lp lc2 gl = ret gvs2 ->
+  OpsemAux.callExternalFunction M1 fid0 gvs1 = ret (oresult1, M1') ->
+  OpsemAux.callExternalFunction M2 fid0 gvs2 = ret (oresult2, M2') ->
+  Opsem.exCallUpdateLocals TD ft noret0 rid oresult1 lc1 = ret lc1' ->
+  Opsem.exCallUpdateLocals TD ft noret0 rid oresult2 lc2 = ret lc2' ->
+  als_simulation pinfo mi F lc1 als1 als2 ->
+  oresult1 = oresult2 /\ 
+  exists mi', 
+    mem_simulation pinfo mgb mi' 
+      ((F,lc1') :: strip_ECs EC) M1' M2' /\ Values.inject_incr mi mi' /\
+    als_simulation pinfo mi' F lc1' als1 als2 /\
+    reg_simulation pinfo mi' F lc1' lc2' /\
+    (forall blk : mblock,
+       ~ isnt_alloca_in_ECs pinfo (strip_ECs EC) blk -> 
+       mi blk = merror -> mi' blk = merror).
+Admitted.
+
+Lemma dae_is_sim : forall maxb pinfo mi Cfg1 St1 Cfg2 St2
+  (Hwfpi: WF_PhiInfo pinfo) 
+  (Hwfgl: sb_ds_gv_inject.wf_globals maxb (OpsemAux.Globals Cfg1)) 
+  (Hinbd: 0 <= maxb) (Hnuse: used_in_fdef (PI_id pinfo) (PI_f pinfo) = false)
+  (Hwfpp: OpsemPP.wf_State Cfg1 St1) 
+  (Hnoalias: Promotability.wf_State maxb pinfo Cfg1 St1) 
+  (Hsim: State_simulation pinfo maxb mi Cfg1 St1 Cfg2 St2),
+  (forall (Hrem: removable_State pinfo St1) St1' tr1 
+     (Hop1: Opsem.sInsn Cfg1 St1 St1' tr1), 
+     exists mi',
+       State_simulation pinfo maxb mi' Cfg1 St1' Cfg2 St2 /\ tr1 = trace_nil /\
+       Values.inject_incr mi mi') /\
+  (forall (Hnrem: ~removable_State pinfo St1) St1' St2' tr1 tr2
+     (Hop2: Opsem.sInsn Cfg2 St2 St2' tr2) 
+     (Hop1: Opsem.sInsn Cfg1 St1 St1' tr1), 
+     exists mi',
+       State_simulation pinfo maxb mi' Cfg1 St1' Cfg2 St2' /\ tr1 = tr2 /\
+       Values.inject_incr mi mi').
+Proof.
+
+Local Opaque inscope_of_tmn inscope_of_cmd.
+
+  intros.
+  split; intros.
+Case "removable state". eapply dae_is_sim_removable_state; eauto.
 
 Case "unremovable state".
+  apply not_removable_State_inv in Hnrem. 
   (sInsn_cases (destruct Hop1) SCase).
 
 SCase "sReturn".
@@ -846,9 +1823,9 @@ Focus.
   repeat_solve.
     eapply returnUpdateLocals_als_simulation; eauto.
 
-    clear - H27 H1 Hlcsim2 Hlcsim2'.
-    eapply returnUpdateLocals_reg_simulation with (lc:=lc); eauto.
-
+    clear - H27 H1 Hlcsim2 Hlcsim2' Hwfgl Hmsim Hneq.
+    eapply returnUpdateLocals_reg_simulation with (lc:=lc); 
+      eauto using mem_simulation__wf_sb_sim.
 Unfocus.
       
 SCase "sReturnVoid".
@@ -869,45 +1846,6 @@ Unfocus.
 
 SCase "sBranch".
 Focus.
-
-Ltac destruct_ctx_other :=
-match goal with
-| Hwfpp : OpsemPP.wf_State
-            {|
-            OpsemAux.CurSystem := _;
-            OpsemAux.CurTargetData := ?TD;
-            OpsemAux.CurProducts := _;
-            OpsemAux.Globals := _;
-            OpsemAux.FunTable := _
-             |} _,
-  Hnoalias : Promotability.wf_State _ _ _ _,
-  Hsim : State_simulation _ _ _ _ _ ?Cfg2 ?St2 ,
-  Hop2 : Opsem.sInsn _ _ _ _ |- _ =>
-  destruct TD as [los nts];
-  destruct Hwfpp as 
-    [Hwfg [HwfSystem [HmInS [_ [
-     [Hreach1 [HBinF1 [HFinPs1 _]]] 
-     [ _ HwfCall'
-     ]]
-    ]]]]; subst;
-  destruct Cfg2 as [S2 TD2 Ps2 gl2 fs2];
-  destruct St2 as [ECs2 M2];
-  simpl in Hsim;
-  destruct Hsim as [EQ1 [Hpsim [Hstksim [EQ2 [EQ3 Hmsim]]]]]; subst;
-  destruct ECs2 as [|[F2 B2 cs2 tmn2 lc2 als2] ECs2]; tinv Hstksim;
-  destruct Hstksim as [Hecsim Hstksim];
-  unfold EC_simulation in Hecsim;
-  destruct Hecsim as 
-      [Hfsim2 [Heq1 [Halsim2 [Hbsim2 
-        [Heq3 [Heq4 [Hlcsim2 Hcssim2]]]]]]]; subst;
-  destruct Hnoalias as 
-    [
-      [[Hinscope' _] [HwfECs' HwfHT]] 
-      [[Hdisjals _] HwfM]
-    ]; simpl in Hdisjals;
-  fold Promotability.wf_ECStack in HwfECs'
-end.
-
   destruct_ctx_other.
   apply cmds_simulation_nil_inv in Hcssim2; subst.
   inv Hop2.
@@ -915,39 +1853,39 @@ end.
 
   assert (block_simulation pinfo F (block_intro l' ps' cs' tmn')
            (block_intro l'0 ps'0 cs'0 tmn'0)) as Hbsim.
-
-Lemma simulation__getOperandValue : forall pinfo maxb mi rm rm2 lc lc2 TD Mem 
-    Mem2 gl F v gv gv',
-  wf_globals maxb gl -> 
-  wf_sb_mi maxb mi Mem Mem2 ->
-  reg_simulation pinfo mi TD gl F rm rm2 lc lc2 ->
-  getOperandValue TD v lc gl = ret gv ->
-  getOperandValue TD v lc2 gl = ret gv' ->
-  gv_inject mi gv gv'.
-
-
-
-
+    destruct Hmsim as [_ [_ Hwf_mi]].
+    eapply simulation__getOperandValue in Hlcsim2; eauto.
+    erewrite simulation__isGVZero in H1; eauto.
     clear - H22 H1 Hfsim2.
-    destruct (isGVZero (los, nts) c); eauto using fdef_sim__block_sim.         
+    destruct (isGVZero (los, nts) c0); eauto using fdef_sim__block_sim.        
   assert (Hbsim':=Hbsim).
   apply block_simulation_inv in Hbsim'.
-  destruct Hbsim' as [Heq1 [Heq2 [Hcssim' Heq5]]]; subst.
+  destruct Hbsim' as [Heq1 [Hpssim' [Hcssim' Heq5]]]; subst.
 
-  assert (lc' = lc'0) as Heq.
-    clear - H2 H23 Hbsim2.
-    eapply switchToNewBasicBlock_sim in Hbsim2; eauto.
+  assert (uniqFdef F) as Huniq. eauto using wf_system__uniqFdef.
+  apply phis_simulation_inv in Hpssim'; auto.
   subst.
 
+  assert (reg_simulation pinfo mi F lc' lc'0) as Hlcsim2'.
+    eapply switchToNewBasicBlock_rsim in Hbsim2; eauto.
+
+  assert (blockInFdefB (block_intro l'0 ps'0 cs' tmn'0) F) as HBinF1'.
+    admit.
+  assert (als_simulation pinfo mi F lc' als als2) as Halsim2'.
+    eapply switchToNewBasicBlock_asim; eauto.
+  exists mi.
   repeat_solve.
     exists l'0. exists ps'0. exists nil. auto.
     exists l'0. exists ps'0. exists nil. auto.
-  
-    clear - H2 Hmsim.
-    eapply mem_simulation_update_locals in Hmsim; simpl; eauto.
-      simpl. intros.
-      admit. (* phis <> palloca *)
 
+    destruct Hmsim as [J1 [J2 J3]].
+    split; auto.
+    split; auto.
+      intros blk J.
+      apply J2.
+      intro J4. apply J.
+      simpl.
+      eapply switchToNewBasicBlock_isnt_alloca_in_ECs; eauto; simpl; eauto. 
 Unfocus.
 
 SCase "sBranch_uncond".
@@ -959,24 +1897,34 @@ Focus.
 
   assert (block_simulation pinfo F (block_intro l' ps' cs' tmn')
            (block_intro l'0 ps'0 cs'0 tmn'0)) as Hbsim.
-    eauto using fdef_sim__block_sim.         
+    eauto using fdef_sim__block_sim.        
   assert (Hbsim':=Hbsim).
   apply block_simulation_inv in Hbsim'.
-  destruct Hbsim' as [Heq1 [Heq2 [Hcssim' Heq5]]]; subst.
+  destruct Hbsim' as [Heq1 [Hpssim' [Hcssim' Heq5]]]; subst.
 
-  assert (lc' = lc'0) as Heq.
-    clear - H0 H17 Hbsim2.
-    eapply switchToNewBasicBlock_sim in Hbsim2; eauto.
+  assert (uniqFdef F) as Huniq. eauto using wf_system__uniqFdef.
+  apply phis_simulation_inv in Hpssim'; auto.
   subst.
 
+  assert (reg_simulation pinfo mi F lc' lc'0) as Hlcsim2'.
+    eapply switchToNewBasicBlock_rsim in Hbsim2; eauto.
+
+  assert (blockInFdefB (block_intro l'0 ps'0 cs' tmn'0) F) as HBinF1'.
+    admit.
+  assert (als_simulation pinfo mi F lc' als als2) as Halsim2'.
+    eapply switchToNewBasicBlock_asim; eauto.
+  exists mi.
   repeat_solve.
     exists l'0. exists ps'0. exists nil. auto.
     exists l'0. exists ps'0. exists nil. auto.
-  
-    clear - H0 Hmsim.
-    eapply mem_simulation_update_locals in Hmsim; simpl; eauto.
-      simpl. intros.
-      admit. (* phis <> palloca *)
+
+    destruct Hmsim as [J1 [J2 J3]].
+    split; auto.
+    split; auto.
+      intros blk J.
+      apply J2.
+      intro J4. apply J. simpl.
+      eapply switchToNewBasicBlock_isnt_alloca_in_ECs; eauto; simpl; eauto. 
 Unfocus.
 
 SCase "sBop". abstract (destruct_ctx_other; dse_is_sim_common_case).
@@ -984,133 +1932,73 @@ SCase "sFBop". abstract (destruct_ctx_other; dse_is_sim_common_case).
 SCase "sExtractValue". abstract (destruct_ctx_other; dse_is_sim_common_case).
 SCase "sInsertValue". abstract (destruct_ctx_other; dse_is_sim_common_case).
 SCase "sMalloc". 
- 
   destruct_ctx_other.
- 
   apply cmds_simulation_nelim_cons_inv in Hcssim2; simpl; auto;
   destruct Hcssim2 as [cs3' [Heq Hcssim2]]; subst;
   inv Hop2; uniq_result.
-
-  assert (mb0 = mb) as EQ.
-    destruct Hmsim as [Hmsim _].
-    apply MemProps.malloc_result in H25.
-    apply MemProps.malloc_result in H2. subst. auto.
-  subst.
+  eapply simulation__getOperandValue with (lc2:=lc2) in H0; 
+    eauto using mem_simulation__wf_sb_sim.
+  eapply mem_simulation__malloc in Hmsim; eauto.
+  destruct Hmsim as [mi' [Hmsim [Hinc [Hprop1 Hprop2]]]].
+  exists mi'.
   repeat_solve.
-
-    destruct Hmsim as [Hmsim1 Hmsim2].
-    split; auto.
-      apply MemProps.nextblock_malloc in H2.
-      apply MemProps.nextblock_malloc in H25.
-      rewrite <- H2. rewrite <- H25. rewrite Hmsim1. auto.
-
-      intros.
-      eapply Hmsim2 with (ptr:=ptr)(ty:=ty)(al:=al); eauto.
-      eapply no_alias_head_tail_update in Hnalias; eauto; simpl; auto.
-        intros. admit. (* id <> palloca *)
-
-        (* two cases, if ptr is mb or not, 
-           malloc_preserves_mload_inv needs to be extended. *)
-        admit. admit.
+    eapply als_simulation___malloc; eauto.
+    eapply reg_simulation___malloc; eauto.
+    eapply inject_incr__preserves__ECs_simulation; eauto.
+      eapply malloc__isnt_alloca_in_ECs; eauto.
+    eapply inject_incr__preserves__ftable_simulation; eauto.
 
 SCase "sFree". 
-
   destruct_ctx_other.
- 
   apply cmds_simulation_nelim_cons_inv in Hcssim2; auto.
   destruct Hcssim2 as [cs3' [Heq Hcssim2]]; subst;
   inv Hop2; uniq_result.
-
+  eapply simulation__getOperandValue with (lc2:=lc2) in H; 
+    eauto using mem_simulation__wf_sb_sim.
+  eapply mem_simulation__free in Hmsim; eauto.
+  exists mi.
   repeat_solve.
-    destruct Hmsim as [Hmsim1 Hmsim2].
-    split; auto.
-      apply MemProps.nextblock_free in H1.
-      apply MemProps.nextblock_free in H22.
-      rewrite <- H1. rewrite <- H22. rewrite Hmsim1. auto.
-
-      intros.
-      eapply Hmsim2 with (ptr:=ptr)(ty:=ty)(al:=al); 
-        eauto using MemProps.free_preserves_mload_inv.
-      eapply no_alias_head_tail_irrel in Hnalias; eauto; simpl; auto.
 
 SCase "sAlloca". 
-
   destruct_ctx_other.
- 
   apply cmds_simulation_nelim_cons_inv in Hcssim2; simpl; auto;
   destruct Hcssim2 as [cs3' [Heq Hcssim2]]; subst;
   inv Hop2; uniq_result.
-
-  assert (mb0 = mb) as EQ.
-    destruct Hmsim as [Hmsim _].
-    apply MemProps.malloc_result in H25.
-    apply MemProps.malloc_result in H2. subst. auto.
-  subst.
+  eapply simulation__getOperandValue with (lc2:=lc2) in H0; 
+    eauto using mem_simulation__wf_sb_sim.
+  eapply mem_simulation__alloca in Hmsim; eauto.
+  destruct Hmsim as [mi' [Hmsim [Hinc [Hprop1 Hprop2]]]].
+  exists mi'.
   repeat_solve.
-
-    destruct Hmsim as [Hmsim1 Hmsim2].
-    split; auto.
-      apply MemProps.nextblock_malloc in H2.
-      apply MemProps.nextblock_malloc in H25.
-      rewrite <- H2. rewrite <- H25. rewrite Hmsim1. auto.
-
-      intros.
-      eapply Hmsim2 with (ptr:=ptr)(ty:=ty)(al:=al); eauto.
-      eapply no_alias_head_tail_update in Hnalias; eauto; simpl; auto.
-        intros.
-        admit. (* if id = palloca, then lc2 cannot contain pid *)
-
-        (* two cases, if ptr is mb or not, 
-           malloc_preserves_mload_inv needs to be extended. *)
-        admit. admit. 
+    eapply als_simulation___alloca; eauto. 
+    eapply reg_simulation___malloc; eauto.
+    eapply inject_incr__preserves__ECs_simulation; eauto.
+      eapply malloc__isnt_alloca_in_ECs; eauto.
+    eapply inject_incr__preserves__ftable_simulation; eauto. 
 
 SCase "sLoad". 
   destruct_ctx_other.
-
   apply cmds_simulation_nelim_cons_inv in Hcssim2; simpl; auto;
   destruct Hcssim2 as [cs3' [Heq Hcssim2]]; subst;
   inv Hop2; uniq_result.
-
-  assert (gv = gv0) as EQ.
-    admit. (* no load from pid *)
-  subst.
+  exists mi.
   repeat_solve.
-
-    eapply mem_simulation_update_locals in Hmsim; simpl; eauto.
-      simpl. intros.
-      admit. (* lid <> pid *)
+    apply als_simulation_update_lc; auto.
+    apply reg_simulation_update_non_palloca; auto.
+      eapply simulation__mload; eauto.
+      eapply simulation__getOperandValue; eauto using mem_simulation__wf_sb_sim.
+    eapply mem_simulation__update_non_palloca; eauto; simpl; eauto.
 
 SCase "sStore". 
-
   destruct_ctx_other.
- 
-  assert (PI_f pinfo = F -> 
-          store_in_cmd (PI_id pinfo) (insn_store sid t v1 v2 align0) = false)
-         as J.
-    clear - Hnrem. simpl in Hnrem.
-    destruct v2; auto.
-    intros. subst.
-    destruct (fdef_dec (PI_f pinfo) (PI_f pinfo)); try congruence.
-    simpl.
-    destruct (id_dec i0 (PI_id pinfo)); subst; auto.
-    destruct (id_dec (PI_id pinfo) (PI_id pinfo)); try congruence.
-    contradict Hnrem; auto.
   apply cmds_simulation_nelim_cons_inv in Hcssim2; auto.
   destruct Hcssim2 as [cs3' [Heq Hcssim2]]; subst;
   inv Hop2; uniq_result.
-
+  exists mi.
   repeat_solve.
-    destruct Hmsim as [Hmsim1 Hmsim2].
-    split; auto.
-      apply MemProps.nextblock_mstore in H3.
-      apply MemProps.nextblock_mstore in H28.
-      rewrite <- H3. rewrite <- H28. rewrite Hmsim1. auto.
-
-      intros.
-      eapply Hmsim2 with (ptr:=ptr)(ty:=ty)(al:=al); eauto.
-      eapply no_alias_head_tail_irrel in Hnalias; eauto; simpl; auto.
-        (* two cases, if ptr overlaps with stored ptr or not *)
-        admit. admit.
+    simpl.
+    eapply simulation__mstore; eauto 
+      using simulation__getOperandValue, mem_simulation__wf_sb_sim.
 
 SCase "sGEP". abstract (destruct_ctx_other; dse_is_sim_common_case).
 SCase "sTrunc". abstract (destruct_ctx_other; dse_is_sim_common_case).
@@ -1120,63 +2008,67 @@ SCase "sIcmp". abstract (destruct_ctx_other; dse_is_sim_common_case).
 SCase "sFcmp". abstract (destruct_ctx_other; dse_is_sim_common_case).
 SCase "sSelect". 
   destruct_ctx_other.
-
   apply cmds_simulation_nelim_cons_inv in Hcssim2; simpl; auto;
   destruct Hcssim2 as [cs3' [Heq Hcssim2]]; subst;
   inv Hop2; uniq_result.
-
+  exists mi.
   repeat_solve.
-    destruct (isGVZero (los,nts) c).
-      eapply mem_simulation_update_locals in Hmsim; simpl; eauto.
-        simpl. intros.
-        admit. (* lid <> pid *)
-      eapply mem_simulation_update_locals in Hmsim; simpl; eauto.
-        simpl. intros.
-        admit. (* lid <> pid *)
+    destruct (isGVZero (los,nts) c);
+      apply als_simulation_update_lc; auto.
+    erewrite simulation__isGVZero; eauto
+      using simulation__getOperandValue, mem_simulation__wf_sb_sim.
+    destruct (isGVZero (los,nts) c0);
+      apply reg_simulation_update_non_palloca; eauto
+        using simulation__getOperandValue, mem_simulation__wf_sb_sim.
+    destruct (isGVZero (los,nts) c);
+      eapply mem_simulation__update_non_palloca; eauto; simpl; eauto.
 
 SCase "sCall".
-
   destruct_ctx_other.
   assert (Hcssim2':=Hcssim2).
   apply cmds_simulation_nelim_cons_inv in Hcssim2; auto.
   destruct Hcssim2 as [cs3' [Heq Hcssim2]]; subst.
-
-  inv Hop2.
+  inv Hop2; uniq_result.
 
   SSCase "SCall".
 
-  uniq_result.
   assert (Hfsim1:=Hpsim).
-  eapply lookupFdefViaPtr__simulation in Hfsim1; eauto.
+  eapply lookupFdefViaPtr__simulation in Hfsim1; eauto
+    using simulation__getOperandValue, mem_simulation__wf_sb_sim.
 
   assert (Hbsim1:=Hfsim1).
   eapply fdef_simulation__entry_block_simulation in Hbsim1; eauto.
   assert (Hbsim1':=Hbsim1).
   apply block_simulation_inv in Hbsim1'.
   destruct Hbsim1' as [Heq' [Hpsim1' [Hcsim1' Htsim1']]]; subst.
+  exists mi.
   repeat_solve.
-    exists l'0. exists ps'0. exists nil. auto.
+    exists l'0. exists ps'. exists nil. auto.
     exists l'0. exists ps'0. exists nil. auto.
 
     apply fdef_simulation_inv in Hfsim1.
-    destruct Hfsim1 as [Heq _]. inv Heq. uniq_result.
-    auto.
+    destruct Hfsim1 as [Hfhsim1 Hbssim1].
+    inv Hfhsim1.
 
-    destruct Hmsim as [Hmsim1 Hmsim2].
+    eapply reg_simulation__initLocals; eauto.
+
+    destruct Hmsim as [Hmsim1 [Hmsim2 Hmsim3]].
     split; auto.
-      intros.
-      eapply Hmsim2 with (ptr:=ptr)(ty:=ty)(al:=al); eauto.
-      clear Hmsim2.
-      apply no_alias_head_tail_cons_and in Hnalias.
-      destruct Hnalias as [Hnalias1 Hnalias2]; auto.
+    split; auto.
+      intros blk J.
+      apply Hmsim2. 
+      intro G. apply J.
+      unfold isnt_alloca_in_ECs in *.
+      intros. simpl in Hin.
+      destruct Hin as [Hin | Hin].
+        subst. simpl. admit.
+        apply G. simpl. auto.
 
   SSCase "sExCall".
 
-  uniq_result.
-
-  clear - H28 H1 Hpsim.
-  eapply lookupFdefViaPtr__simulation_l2r in H1; eauto.
-  destruct H1 as [f2 [H1 H2]].
+  eapply lookupFdefViaPtr__simulation_l2r in H1; eauto
+    using simulation__getOperandValue, mem_simulation__wf_sb_sim.
+  destruct H1 as [f2 [H1 H1']].
   apply OpsemAux.lookupExFdecViaPtr_inversion in H28.
   apply OpsemAux.lookupFdefViaPtr_inversion in H1.
   destruct H28 as [fn [J1 [J2 J3]]].
@@ -1189,15 +2081,12 @@ SCase "sExCall".
   assert (Hcssim2':=Hcssim2).
   apply cmds_simulation_nelim_cons_inv in Hcssim2; auto.
   destruct Hcssim2 as [cs3' [Heq Hcssim2]]; subst.
-
-  inv Hop2.
+  inv Hop2; uniq_result.
 
   SSCase "SCall".
 
-  uniq_result.
-
-  clear - H29 H1 Hpsim.
-  eapply lookupExFdecViaPtr__simulation_l2r in H1; eauto.
+  eapply lookupExFdecViaPtr__simulation_l2r in H1; eauto
+    using simulation__getOperandValue, mem_simulation__wf_sb_sim.
   apply OpsemAux.lookupExFdecViaPtr_inversion in H1.
   apply OpsemAux.lookupFdefViaPtr_inversion in H29.
   destruct H1 as [fn [J1 [J2 J3]]].
@@ -1206,17 +2095,16 @@ SCase "sExCall".
 
   SSCase "sExCall".
 
+  eapply lookupExFdecViaPtr__simulation_l2r in H1; eauto
+    using simulation__getOperandValue, mem_simulation__wf_sb_sim.
   uniq_result.
 
-  assert (Hlkdec:=Hpsim).
-  eapply lookupExFdecViaPtr__simulation_l2r in Hlkdec; eauto.
-  uniq_result.
-  eapply callExternalFunction__Mem_simulation in Hmsim; eauto.
-  destruct Hmsim as [EQ Hmsim]; subst.
-  uniq_result.
+  eapply callExternalFunction__mem_simulation in Hmsim; eauto.
+  destruct Hmsim as [EQ [mi' [Hmsim [Hinc [J1 [J2 J3]]]]]]; subst.
+  exists mi'.
   repeat_solve.
-    eapply mem_simulation_update_locals in Hmsim; simpl; eauto.
-      simpl. intros. admit. (* cid <> pid *)
+    eapply inject_incr__preserves__ECs_simulation; eauto.
+    eapply inject_incr__preserves__ftable_simulation; eauto.
     
 Transparent inscope_of_tmn inscope_of_cmd.
 
