src/SoftBound/sb_ds_trans_lib.v
@@ -190,48 +190,6 @@ Proof.
   eapply simulation__mfbop in H3; eauto.
 Qed.
 
-Lemma simulation__GEP : forall maxb mi TD Mem Mem2 inbounds0 vidxs vidxs' gvp1 
-    gvp gvp' t,
-  wf_sb_mi maxb mi Mem Mem2 ->
-  gv_inject mi gvp gvp' ->
-  gvs_inject mi vidxs vidxs' ->
-  GEP TD t gvp vidxs inbounds0 = ret gvp1 ->
-  exists gvp2,
-    GEP TD t gvp' vidxs' inbounds0 = ret gvp2 /\
-    gv_inject mi gvp1 gvp2.
-Proof.
-  intros maxb mi TD Mem Mem2 inbounds0 vidxs vidxs' gvp1 gvp gvp' t H H0 H1 H2.
-  unfold GEP in *.
-  remember (GV2ptr TD (getPointerSize TD) gvp) as R.
-  destruct R; inv H2.
-    symmetry in HeqR.
-    eapply simulation__GV2ptr in HeqR; eauto.
-    destruct HeqR as [v' [J1 J2]].
-    rewrite J1. 
-    assert (GVs2Nats TD vidxs = GVs2Nats TD vidxs') as EQ.
-      eapply simulation__GVs2Nats; eauto.
-    rewrite <- EQ.
-    destruct (GVs2Nats TD vidxs).
-      remember (mgep TD t v l0) as R1.
-      destruct R1; inv H4.
-        symmetry in HeqR1.
-        eapply simulation__mgep in HeqR1; eauto.
-        destruct HeqR1 as [v0' [J11 J12]].
-        rewrite J11. exists (ptr2GV TD v0').
-        unfold ptr2GV, val2GV.
-        simpl. eauto.
-
-        symmetry in HeqR1.
-        eapply simulation__mgep' in HeqR1; eauto.
-        rewrite HeqR1. rewrite H3.
-        eauto using gv_inject_gundef.
-
-      rewrite H4. eauto using gv_inject_gundef.
-
-    erewrite simulation__GV2ptr'; eauto.
-    rewrite H4. eauto using gv_inject_gundef.
-Qed.
-
 Lemma simulation__values2GVs : forall maxb mi rm rm2 lc lc2 TD Mem Mem2 
     gl F idxs gvs,
   wf_globals maxb gl -> 
@@ -2792,7 +2750,7 @@ Qed.
 (*
 *** Local Variables: ***
 *** coq-prog-name: "coqtop" ***
-*** coq-prog-args: ("-emacs-U" "-I" "~/SVN/sol/vol/src/Vellvm/monads" "-I" "~/SVN/sol/vol/src/Vellvm/ott" "-I" "~/SVN/sol/vol/src/Vellvm/compcert" "-I" "~/SVN/sol/theory/metatheory_8.3" "-I" "~/SVN/sol/vol/src/TV" "-impredicative-set") ***
+*** coq-prog-args: ("-emacs-U" "-I" "~/SVN/sol/vol/src/Vellvm/monads" "-I" "~/SVN/sol/vol/src/Vellvm/ott" "-I" "~/SVN/sol/vol/src/Vellvm/compcert" "-I" "~/SVN/sol/theory/metatheory_8.3" "-impredicative-set") ***
 *** End: ***
  *)
 
